Write ltamer-based CPS transform

src/Experiments/SimplyTypedArithmetic.v
@@ -138,8 +138,8 @@ Module Positional. Section Positional.
     rewrite <- (seq_length n 0) at 2.
     generalize dependent (List.seq 0 n); intro xs.
     induction xs; simpl; nsatz.                               Qed.
-  Definition add_to_nth i x : list Z -> list Z
-    := ListUtil.update_nth i (runtime_add x).
+  Definition add_to_nth i x (ls : list Z) : list Z
+    := ListUtil.update_nth i (fun y => runtime_add x y) ls.
   Lemma eval_add_to_nth (n:nat) (i:nat) (x:Z) (xs:list Z) (H:(i<length xs)%nat)
         (Hn : length xs = n) (* N.B. We really only need [i < Nat.min n (length xs)] *) :
     eval n (add_to_nth i x xs) = weight i * x + eval n xs.
@@ -179,9 +179,9 @@ Module Positional. Section Positional.
   Hint Rewrite weight_place : push_eval.
 
   Definition from_associational n (p:list (Z*Z)) :=
-    List.fold_right (fun t =>
+    List.fold_right (fun t ls =>
       let p := place t (pred n) in
-      add_to_nth (fst p) (snd p)    ) (zeros n) p.
+      add_to_nth (fst p) (snd p) ls ) (zeros n) p.
   Lemma eval_from_associational {n} p (n_nz:n<>O \/ p = nil) :
     eval n (from_associational n p) = Associational.eval p.
   Proof. destruct n_nz; [ induction p | subst p ];
@@ -254,7 +254,7 @@ Module Positional. Section Positional.
 
       will produce [fun a b c d => (a + (b + (c + d)))].*)
     Definition chained_carries {n} s c p (idxs : list nat) :=
-      fold_right (@carry_reduce n s c) p (rev idxs).
+      fold_right (fun a b => @carry_reduce n s c a b) p (rev idxs).
 
     Lemma eval_chained_carries {n} s c p idxs :
       (s <> 0) -> (s - Associational.eval c <> 0) -> (n <> 0%nat) ->
@@ -340,78 +340,122 @@ Module Compilers.
   End type.
   Export type.Notations.
 
-  Module expr.
-    Inductive expr {ident : type -> Type} {var : type -> Type} : type -> Type :=
-    | Var {t} (v : var t) : expr t
-    | Ident {t} (idc : ident t) : expr t
-    | App {s d} (f : expr (s -> d)) (x : expr s) : expr d
-    | Abs {s d} (f : var s -> expr d) : expr (s -> d).
+  Module Uncurried.
+    Module expr.
+      Inductive expr {ident : type -> type -> Type} {var : type -> Type} : type -> Type :=
+      | Var {t} (v : var t) : expr t
+      | TT : expr type.unit
+      | AppIdent {s d} (idc : ident s d) (args : expr s) : expr d
+      | App {s d} (f : expr (s -> d)) (x : expr s) : expr d
+      | Pair {A B} (a : expr A) (b : expr B) : expr (A * B)
+      | Abs {s d} (f : var s -> expr d) : expr (s -> d).
 
-    Module Export Notations.
-      Bind Scope expr_scope with expr.
-      Delimit Scope expr_scope with expr.
+      Module Export Notations.
+        Bind Scope expr_scope with expr.
+        Delimit Scope expr_scope with expr.
 
-      Infix "@" := App : expr_scope.
-      Notation "'λ'  x .. y , t" := (Abs (fun x => .. (Abs (fun y => t%expr)) ..)) : expr_scope.
-    End Notations.
+        Infix "@" := App : expr_scope.
+        Infix "@@" := AppIdent : expr_scope.
+        Notation "( x , y , .. , z )" := (Pair .. (Pair x%expr y%expr) .. z%expr) : expr_scope.
+        Notation "( )" := TT : expr_scope.
+        Notation "()" := TT : expr_scope.
+        Notation "'λ'  x .. y , t" := (Abs (fun x => .. (Abs (fun y => t%expr)) ..)) : expr_scope.
+      End Notations.
 
-    Definition Expr {ident : type -> Type} t := forall var, @expr ident var t.
+      Definition Expr {ident : type -> type -> Type} t := forall var, @expr ident var t.
 
-    Section with_ident.
-      Context {ident : type -> Type}
-              (interp_ident : forall t, ident t -> type.interp t).
+      Section unexpr.
+        Context {ident : type -> type -> Type}
+                {var : type -> Type}.
 
-      Fixpoint interp {t} (e : @expr ident type.interp t) : type.interp t
-        := match e with
-           | Var t v => v
-           | Ident t idc => interp_ident t idc
-           | App s d f x => interp f (interp x)
-           | Abs s d f => fun v => interp (f v)
-           end.
+        Fixpoint unexpr {t} (e : @expr ident (@expr ident var) t) : @expr ident var t
+          := match e in expr t return expr t with
+             | Var t v => v
+             | TT => TT
+             | AppIdent s d idc args => AppIdent idc (unexpr args)
+             | App s d f x => App (unexpr f) (unexpr x)
+             | Pair A B a b => Pair (unexpr a) (unexpr b)
+             | Abs s d f => Abs (fun x => unexpr (f (Var x)))
+             end.
+      End unexpr.
 
-      Definition Interp {t} (e : Expr t) := interp (e _).
-    End with_ident.
+      Section with_ident.
+        Context {ident : type -> type -> Type}
+                (interp_ident : forall s d, ident s d -> type.interp s -> type.interp d).
 
-    Ltac is_primitive_const_cps2 term on_success on_failure :=
-      let recurse term := is_primitive_const_cps2 term on_success on_failure in
-      lazymatch term with
-      | S ?n => recurse n
-      | O => on_success ()
-      | true => on_success ()
-      | false => on_success ()
-      | tt => on_success ()
-      | Z0 => on_success ()
-      | Zpos ?p => recurse p
-      | Zneg ?p => recurse p
-      | xI ?p => recurse p
-      | xO ?p => recurse p
-      | xH => on_success ()
-      | ?term => on_failure term
-      end.
-    Ltac require_primitive_const term :=
-      is_primitive_const_cps2 term ltac:(fun _ => idtac) ltac:(fun term => fail 0 "Not a known const:" term).
-    Ltac is_primitive_const term :=
-      is_primitive_const_cps2 term ltac:(fun _ => true) ltac:(fun _ => false).
+        Fixpoint interp {t} (e : @expr ident type.interp t) : type.interp t
+          := match e with
+             | Var t v => v
+             | TT => tt
+             | AppIdent s d idc args => interp_ident s d idc (@interp s args)
+             | App s d f x => @interp _ f (@interp _ x)
+             | Pair A B a b => (@interp A a, @interp B b)
+             | Abs s d f => fun v => interp (f v)
+             end.
 
-    Module var_context.
-      Inductive list {var : type -> Type} :=
-      | nil
-      | cons {t} (gallina_v : type.interp t) (v : var t) (ctx : list).
-    End var_context.
+        Definition Interp {t} (e : Expr t) := interp (e _).
+      End with_ident.
 
-    (* cf COQBUG(https://github.com/coq/coq/issues/5448) , COQBUG(https://github.com/coq/coq/issues/6315) *)
-    Ltac refresh n :=
-      let n' := fresh n in
-      let n' := fresh n in
-      n'.
+      Ltac is_primitive_const_cps2 term on_success on_failure :=
+        let recurse term := is_primitive_const_cps2 term on_success on_failure in
+        lazymatch term with
+        | S ?n => recurse n
+        | O => on_success ()
+        | true => on_success ()
+        | false => on_success ()
+        | tt => on_success ()
+        | Z0 => on_success ()
+        | Zpos ?p => recurse p
+        | Zneg ?p => recurse p
+        | xI ?p => recurse p
+        | xO ?p => recurse p
+        | xH => on_success ()
+        | ?term => on_failure term
+        end.
+      Ltac require_primitive_const term :=
+        is_primitive_const_cps2 term ltac:(fun _ => idtac) ltac:(fun term => fail 0 "Not a known const:" term).
+      Ltac is_primitive_const term :=
+        is_primitive_const_cps2 term ltac:(fun _ => true) ltac:(fun _ => false).
 
-    Ltac type_of_first_argument_of f :=
-      let f_ty := type of f in
-      lazymatch eval hnf in f_ty with
-      | forall x : ?T, _ => T
-      end.
+      Module var_context.
+        Inductive list {var : type -> Type} :=
+        | nil
+        | cons {t} (gallina_v : type.interp t) (v : var t) (ctx : list).
+      End var_context.
 
-    (** Forms of abstraction in Gallina that our reflective language
+      (* cf COQBUG(https://github.com/coq/coq/issues/5448) , COQBUG(https://github.com/coq/coq/issues/6315) , COQBUG(https://github.com/coq/coq/issues/6559) *)
+      Ltac require_same_var n1 n2 :=
+        (*idtac n1 n2;*)
+        let c1 := constr:(fun n1 n2 : Set => ltac:(exact n1)) in
+        let c2 := constr:(fun n1 n2 : Set => ltac:(exact n2)) in
+        (*idtac c1 c2;*)
+        first [ constr_eq c1 c2 | fail 1 "Not the same var:" n1 "and" n2 "(via constr_eq" c1 c2 ")" ].
+      Ltac is_same_var n1 n2 :=
+        match goal with
+        | _ => let check := match goal with _ => require_same_var n1 n2 end in
+               true
+        | _ => false
+        end.
+      Ltac is_underscore v :=
+        let v' := fresh v in
+        let v' := fresh v' in
+        is_same_var v v'.
+      Ltac refresh n fresh_tac :=
+        let n_is_underscore := is_underscore n in
+        let n' := lazymatch n_is_underscore with
+                  | true => fresh
+                  | false => fresh_tac n
+                  end in
+        let n' := fresh_tac n' in
+        n'.
+
+      Ltac type_of_first_argument_of f :=
+        let f_ty := type of f in
+        lazymatch eval hnf in f_ty with
+        | forall x : ?T, _ => T
+        end.
+
+      (** Forms of abstraction in Gallina that our reflective language
       cannot handle get handled by specializing the code "template" to
       each particular application of that abstraction. In particular,
       type arguments (nat, Z, (λ _, nat), etc) get substituted into
@@ -420,74 +464,74 @@ Module Compilers.
       reification, we accumulate them in a right-associated tuple,
       using [tt] as the "nil" base case.  When we hit a λ or an
       identifier, we plug in the template parameters as necessary. *)
-    Ltac require_template_parameter parameter_type :=
-      first [ unify parameter_type Prop
-            | unify parameter_type Set
-            | unify parameter_type Type
-            | lazymatch eval hnf in parameter_type with
-              | forall x : ?T, @?P x
-                => let check := constr:(fun x : T
-                                        => ltac:(require_template_parameter (P x);
-                                                 exact I)) in
-                   idtac
-              end ].
-    Ltac is_template_parameter parameter_type :=
-      is_success_run_tactic ltac:(fun _ => require_template_parameter parameter_type).
-    Ltac plug_template_ctx f template_ctx :=
-      lazymatch template_ctx with
-      | tt => f
-      | (?arg, ?template_ctx')
-        =>
-        let T := type_of_first_argument_of f in
-        let x_is_template_parameter := is_template_parameter T in
-        lazymatch x_is_template_parameter with
-        | true
-          => plug_template_ctx (f arg) template_ctx'
-        | false
-          => constr:(fun x : T
-                     => ltac:(let v := plug_template_ctx (f x) template_ctx in
-                              exact v))
-        end
-      end.
+      Ltac require_template_parameter parameter_type :=
+        first [ unify parameter_type Prop
+              | unify parameter_type Set
+              | unify parameter_type Type
+              | lazymatch eval hnf in parameter_type with
+                | forall x : ?T, @?P x
+                  => let check := constr:(fun x : T
+                                          => ltac:(require_template_parameter (P x);
+                                                   exact I)) in
+                     idtac
+                end ].
+      Ltac is_template_parameter parameter_type :=
+        is_success_run_tactic ltac:(fun _ => require_template_parameter parameter_type).
+      Ltac plug_template_ctx f template_ctx :=
+        lazymatch template_ctx with
+        | tt => f
+        | (?arg, ?template_ctx')
+          =>
+          let T := type_of_first_argument_of f in
+          let x_is_template_parameter := is_template_parameter T in
+          lazymatch x_is_template_parameter with
+          | true
+            => plug_template_ctx (f arg) template_ctx'
+          | false
+            => constr:(fun x : T
+                       => ltac:(let v := plug_template_ctx (f x) template_ctx in
+                                exact v))
+          end
+        end.
 
-    Ltac reify_helper ident reify_ident var term value_ctx template_ctx :=
-      let reify_rec_gen term value_ctx template_ctx := reify_helper ident reify_ident var term value_ctx template_ctx in
-      let reify_rec term := reify_rec_gen term value_ctx template_ctx in
-      (*let dummy := match goal with _ => idtac "reify_helper: attempting to reify:" term end in*)
-      lazymatch value_ctx with
-      | context[@var_context.cons _ ?rT term ?v _]
-        => constr:(@Var ident var rT v)
-      | _
-        =>
-        let term_is_primitive_const := is_primitive_const term in
-        lazymatch term_is_primitive_const with
-        | true
-          => let rv := reify_ident term in
-             constr:(Ident (var:=var) rv)
-        | false
+      Ltac reify_helper ident reify_ident var term value_ctx template_ctx :=
+        let reify_rec_gen term value_ctx template_ctx := reify_helper ident reify_ident var term value_ctx template_ctx in
+        let reify_rec term := reify_rec_gen term value_ctx template_ctx in
+        let reify_rec_not_head term := reify_rec_gen term value_ctx tt in
+        let mkAppIdent idc args
+            := let rargs := reify_rec_not_head args in
+               constr:(@AppIdent ident var _ _ idc rargs) in
+        let do_reify_ident term else_tac
+            := let term_is_primitive_const := is_primitive_const term in
+               reify_ident
+                 mkAppIdent
+                 term_is_primitive_const
+                 term
+                 else_tac in
+        (*let dummy := match goal with _ => idtac "reify_helper: attempting to reify:" term end in*)
+        lazymatch value_ctx with
+        | context[@var_context.cons _ ?rT term ?v _]
+          => constr:(@Var ident var rT v)
+        | _
           =>
           lazymatch term with
           | match ?b with true => ?t | false => ?f end
             => let T := type of t in
                reify_rec (@bool_rect (fun _ => T) t f b)
+          | match ?x with Datatypes.pair a b => ?f end
+            => reify_rec (match Datatypes.fst x, Datatypes.snd x return _ with
+                          | a, b => f
+                          end)
           | let x := ?a in @?b x
             => let A := type of a in
                let B := lazymatch type of b with forall x, @?B x => B end in
                reify_rec (@Let_In A B a b)
-          | ?f ?x
-            =>
-            let ty := type_of_first_argument_of f in
-            let x_is_template_parameter := is_template_parameter ty in
-            lazymatch x_is_template_parameter with
-            | true
-              => (* we can't reify things of type [Type], so we save it for later to plug in *)
-              reify_rec_gen f value_ctx (x, template_ctx)
-            | false
-              =>
-              let rx := reify_rec_gen x value_ctx tt in
-              let rf := reify_rec_gen f value_ctx template_ctx in
-              constr:(App (var:=var) rf rx)
-            end
+          | Datatypes.pair ?x ?y
+            => let rx := reify_rec x in
+               let ry := reify_rec y in
+               constr:(Pair (ident:=ident) (var:=var) rx ry)
+          | tt
+            => constr:(@TT ident var)
           | (fun x : ?T => ?f)
             =>
             let x_is_template_parameter := is_template_parameter T in
@@ -502,9 +546,10 @@ Module Compilers.
             | false
               =>
               let rT := type.reify T in
-              let not_x := refresh x in
-              let not_x2 := refresh not_x in
-              let not_x3 := refresh not_x2 in
+              let not_x := refresh x ltac:(fun n => fresh n) in
+              let not_x2 := refresh not_x ltac:(fun n => fresh n) in
+              let not_x3 := refresh not_x2 ltac:(fun n => fresh n) in
+              (*let dummy := match goal with _ => idtac "reify_helper: λ case:" term "using vars:" not_x not_x2 not_x3 end in*)
               let rf0 :=
                   constr:(
                     fun (x : T) (not_x : var rT)
@@ -535,593 +580,703 @@ Module Compilers.
               end
             end
           | _
-            => let term := plug_template_ctx term template_ctx in
-               let idc := reify_ident term in
-               constr:(Ident (var:=var) idc)
+            =>
+            do_reify_ident
+              term
+              ltac:(
+              fun _
+              =>
+                lazymatch term with
+                | ?f ?x
+                  =>
+                  let ty := type_of_first_argument_of f in
+                  let x_is_template_parameter := is_template_parameter ty in
+                  lazymatch x_is_template_parameter with
+                  | true
+                    => (* we can't reify things of type [Type], so we save it for later to plug in *)
+                    reify_rec_gen f value_ctx (x, template_ctx)
+                  | false
+                    => let rx := reify_rec_gen x value_ctx tt in
+                       let rf := reify_rec_gen f value_ctx template_ctx in
+                       constr:(App (ident:=ident) (var:=var) rf rx)
+                  end
+                | _
+                  => let term := plug_template_ctx term template_ctx in
+                     do_reify_ident
+                       term
+                       ltac:(fun _
+                             => let dummy := match goal with
+                                             | _ => fail 1 "Unrecognized term:" term
+                                             end in
+                                constr:(I : I))
+                end)
           end
-        end
-      end.
-    Ltac reify ident reify_ident var term :=
-      reify_helper ident reify_ident var term (@var_context.nil var) tt.
-    Ltac Reify ident reify_ident term :=
-      constr:(fun var : type -> Type
-              => ltac:(let r := reify ident reify_ident var term in
-                       exact r)).
-    Ltac Reify_rhs ident reify_ident interp_ident _ :=
-      let RHS := lazymatch goal with |- _ = ?RHS => RHS end in
-      let R := Reify ident reify_ident RHS in
-      transitivity (@Interp ident interp_ident _ R);
-      [ | cbv beta iota delta [Interp interp interp_ident Let_In type.interp bool_rect];
-          reflexivity ].
+        end.
+      Ltac reify ident reify_ident var term :=
+        reify_helper ident reify_ident var term (@var_context.nil var) tt.
+      Ltac Reify ident reify_ident term :=
+        constr:(fun var : type -> Type
+                => ltac:(let r := reify ident reify_ident var term in
+                         exact r)).
+      Ltac Reify_rhs ident reify_ident interp_ident _ :=
+        let RHS := lazymatch goal with |- _ = ?RHS => RHS end in
+        let R := Reify ident reify_ident RHS in
+        transitivity (@Interp ident interp_ident _ R);
+        [ | cbv beta iota delta [Interp interp interp_ident Let_In type.interp bool_rect];
+            reflexivity ].
 
-    Module for_reification.
-      Module ident.
-        Import type.
-        Inductive ident : type -> Set :=
-        | primitive {t:type.primitive} (v : interp t) : ident t
-        | Let_In {tx tC} : ident (tx -> (tx -> tC) -> tC)
-        | Nat_succ : ident (nat -> nat)
-        | nil {t} : ident (list t)
-        | cons {t} : ident (t -> list t -> list t)
-        | pair {A B} : ident (A -> B -> A * B)
-        | fst {A B} : ident (A * B -> A)
-        | snd {A B} : ident (A * B -> B)
-        | bool_rect {T} : ident (T -> T -> bool -> T)
-        | nat_rect {P} : ident (P -> (nat -> P -> P) -> nat -> P)
-        | pred : ident (nat -> nat)
-        | List_seq : ident (nat -> nat -> list nat)
-        | List_repeat {A} : ident (A -> nat -> list A)
-        | List_combine {A B} : ident (list A -> list B -> list (A * B))
-        | List_map {A B} : ident ((A -> B) -> list A -> list B)
-        | List_flat_map {A B} : ident ((A -> list B) -> list A -> list B)
-        | List_partition {A} : ident ((A -> bool) -> list A -> list A * list A)
-        | List_app {A} : ident (list A -> list A -> list A)
-        | List_rev {A} : ident (list A -> list A)
-        | List_fold_right {A B} : ident ((B -> A -> A) -> A -> list B -> A)
-        | List_update_nth {T} : ident (nat -> (T -> T) -> list T -> list T)
-        | List_nth_default {T} : ident (T -> list T -> nat -> T)
-        | Z_runtime_mul : ident (Z -> Z -> Z)
-        | Z_runtime_add : ident (Z -> Z -> Z)
-        | Z_add : ident (Z -> Z -> Z)
-        | Z_mul : ident (Z -> Z -> Z)
-        | Z_pow : ident (Z -> Z -> Z)
-        | Z_opp : ident (Z -> Z)
-        | Z_div : ident (Z -> Z -> Z)
-        | Z_modulo : ident (Z -> Z -> Z)
-        | Z_eqb : ident (Z -> Z -> bool)
-        | Z_of_nat : ident (nat -> Z).
+      Module for_reification.
+        Module ident.
+          Import type.
+          Inductive ident : type -> type -> Set :=
+          | primitive {t:type.primitive} (v : interp t) : ident () t
+          | Let_In {tx tC} : ident (tx * (tx -> tC)) tC
+          | Nat_succ : ident nat nat
+          | nil {t} : ident () (list t)
+          | cons {t} : ident (t * list t) (list t)
+          | fst {A B} : ident (A * B) A
+          | snd {A B} : ident (A * B) B
+          | bool_rect {T} : ident (T * T * bool) T
+          | nat_rect {P} : ident (P * (nat * P -> P) * nat) P
+          | pred : ident nat nat
+          | List_seq : ident (nat * nat) (list nat)
+          | List_repeat {A} : ident (A * nat) (list A)
+          | List_combine {A B} : ident (list A * list B) (list (A * B))
+          | List_map {A B} : ident ((A -> B) * list A) (list B)
+          | List_flat_map {A B} : ident ((A -> list B) * list A) (list B)
+          | List_partition {A} : ident ((A -> bool) * list A) (list A * list A)
+          | List_app {A} : ident (list A * list A) (list A)
+          | List_rev {A} : ident (list A) (list A)
+          | List_fold_right {A B} : ident ((B * A -> A) * A * list B) A
+          | List_update_nth {T} : ident (nat * (T -> T) * list T) (list T)
+          | List_nth_default {T} : ident (T * list T * nat) T
+          | Z_runtime_mul : ident (Z * Z) Z
+          | Z_runtime_add : ident (Z * Z) Z
+          | Z_add : ident (Z * Z) Z
+          | Z_mul : ident (Z * Z) Z
+          | Z_pow : ident (Z * Z) Z
+          | Z_opp : ident Z Z
+          | Z_div : ident (Z * Z) Z
+          | Z_modulo : ident (Z * Z) Z
+          | Z_eqb : ident (Z * Z) bool
+          | Z_of_nat : ident nat Z.
 
-        Definition interp {t} (idc : ident t) : type.interp t
-          := match idc in ident t return type.interp t with
-             | primitive _ v => v
-             | Let_In tx tC => @LetIn.Let_In (type.interp tx) (fun _ => type.interp tC)
-             | Nat_succ => Nat.succ
-             | nil t => @Datatypes.nil (type.interp t)
-             | cons t => @Datatypes.cons (type.interp t)
-             | pair A B => @Datatypes.pair (type.interp A) (type.interp B)
-             | fst A B => @Datatypes.fst (type.interp A) (type.interp B)
-             | snd A B => @Datatypes.snd (type.interp A) (type.interp B)
-             | bool_rect T => @Datatypes.bool_rect (fun _ => type.interp T)
-             | nat_rect P => @Datatypes.nat_rect (fun _ => type.interp P)
-             | pred => Nat.pred
-             | List_seq => List.seq
-             | List_combine A B => @List.combine (type.interp A) (type.interp B)
-             | List_map A B => @List.map (type.interp A) (type.interp B)
-             | List_repeat A => @List.repeat (type.interp A)
-             | List_flat_map A B => @List.flat_map (type.interp A) (type.interp B)
-             | List_partition A => @List.partition (type.interp A)
-             | List_app A => @List.app (type.interp A)
-             | List_rev A => @List.rev (type.interp A)
-             | List_fold_right A B => @List.fold_right (type.interp A) (type.interp B)
-             | List_update_nth T => @update_nth (type.interp T)
-             | List_nth_default T => @List.nth_default (type.interp T)
-             | Z_runtime_mul => runtime_mul
-             | Z_runtime_add => runtime_add
-             | Z_add => Z.add
-             | Z_mul => Z.mul
-             | Z_pow => Z.pow
-             | Z_modulo => Z.modulo
-             | Z_opp => Z.opp
-             | Z_div => Z.div
-             | Z_eqb => Z.eqb
-             | Z_of_nat => Z.of_nat
-             end.
+          Notation curry0 f
+            := (fun 'tt => f).
+          Notation curry2 f
+            := (fun '(a, b) => f a b).
+          Notation curry3 f
+            := (fun '(a, b, c) => f a b c).
+          Notation uncurry2 f
+            := (fun a b => f (a, b)).
+          Notation curry3_1 f
+            := (fun '(a, b, c) => f (uncurry2 a) b c).
+          Notation curry3_2 f
+            := (fun '(a, b, c) => f a (uncurry2 b) c).
 
-        Ltac reify term :=
-          (*let dummy := match goal with _ => idtac "attempting to reify_op" term end in*)
-          lazymatch term with
-          | Nat.succ => Nat_succ
-          | S => Nat_succ
-          | @Datatypes.nil ?T
-            => let rT := type.reify T in
-               constr:(@ident.nil rT)
-          | @Datatypes.cons ?T
-            => let rT := type.reify T in
-               constr:(@ident.cons rT)
-          | @Datatypes.pair ?A ?B
-            => let rA := type.reify A in
-               let rB := type.reify B in
-               constr:(@ident.pair rA rB)
-          | @Datatypes.fst ?A ?B
-            => let rA := type.reify A in
-               let rB := type.reify B in
-               constr:(@ident.fst rA rB)
-          | @Datatypes.snd ?A ?B
-            => let rA := type.reify A in
-               let rB := type.reify B in
-               constr:(@ident.snd rA rB)
-          | @Datatypes.bool_rect (fun _ => ?T)
-            => let rT := type.reify T in
-               constr:(@ident.bool_rect rT)
-          | @Datatypes.nat_rect (fun _ => ?T)
-            => let rT := type.reify T in
-               constr:(@ident.nat_rect rT)
-          | Nat.pred => ident.pred
-          | List.seq => ident.List_seq
-          | @List.repeat ?A
-            => let rA := type.reify A in
-               constr:(@ident.List_repeat rA)
-          | @LetIn.Let_In ?A (fun _ => ?B)
-            => let rA := type.reify A in
-               let rB := type.reify B in
-               constr:(@ident.Let_In rA rB)
-          | @LetIn.Let_In ?A ?B
-            => let dummy := match goal with _ => fail 1 "Let_In contains a dependent type λ as its second argument:" B end in
-               constr:(I : I)
-          | @combine ?A ?B
-            => let rA := type.reify A in
-               let rB := type.reify B in
-               constr:(@ident.List_combine rA rB)
-          | @List.map ?A ?B
-            => let rA := type.reify A in
-               let rB := type.reify B in
-               constr:(@ident.List_map rA rB)
-          | @List.flat_map ?A ?B
-            => let rA := type.reify A in
-               let rB := type.reify B in
-               constr:(@ident.List_flat_map rA rB)
-          | @List.partition ?A
-            => let rA := type.reify A in
-               constr:(@ident.List_partition rA)
-          | @List.app ?A
-            => let rA := type.reify A in
-               constr:(@ident.List_app rA)
-          | @List.rev ?A
-            => let rA := type.reify A in
-               constr:(@ident.List_rev rA)
-          | @List.fold_right ?A ?B
-            => let rA := type.reify A in
-               let rB := type.reify B in
-               constr:(@ident.List_fold_right rA rB)
-          | @update_nth ?T
-            => let rT := type.reify T in
-               constr:(@ident.List_update_nth rT)
-          | @List.nth_default ?T
-            => let rT := type.reify T in
-               constr:(@ident.List_nth_default rT)
-          | runtime_mul => ident.Z_runtime_mul
-          | runtime_add => ident.Z_runtime_add
-          | Z.add => ident.Z_add
-          | Z.mul => ident.Z_mul
-          | Z.pow => ident.Z_pow
-          | Z.opp => ident.Z_opp
-          | Z.div => ident.Z_div
-          | Z.modulo => ident.Z_modulo
-          | Z.eqb => ident.Z_eqb
-          | Z.of_nat => ident.Z_of_nat
-          | _
-            => let assert_const := match goal with
-                                   | _ => require_primitive_const term
-                                   end in
-               let T := type of term in
-               let rT := type.reify_primitive T in
-               constr:(@ident.primitive rT term)
-          end.
+          Definition interp {s d} (idc : ident s d) : type.interp s -> type.interp d
+            := match idc in ident s d return type.interp s -> type.interp d with
+               | primitive _ v => curry0 v
+               | Let_In tx tC => curry2 (@LetIn.Let_In (type.interp tx) (fun _ => type.interp tC))
+               | Nat_succ => Nat.succ
+               | nil t => curry0 (@Datatypes.nil (type.interp t))
+               | cons t => curry2 (@Datatypes.cons (type.interp t))
+               | fst A B => @Datatypes.fst (type.interp A) (type.interp B)
+               | snd A B => @Datatypes.snd (type.interp A) (type.interp B)
+               | bool_rect T => curry3 (@Datatypes.bool_rect (fun _ => type.interp T))
+               | nat_rect P => curry3_2 (@Datatypes.nat_rect (fun _ => type.interp P))
+               | pred => Nat.pred
+               | List_seq => curry2 List.seq
+               | List_combine A B => curry2 (@List.combine (type.interp A) (type.interp B))
+               | List_map A B => curry2 (@List.map (type.interp A) (type.interp B))
+               | List_repeat A => curry2 (@List.repeat (type.interp A))
+               | List_flat_map A B => curry2 (@List.flat_map (type.interp A) (type.interp B))
+               | List_partition A => curry2 (@List.partition (type.interp A))
+               | List_app A => curry2 (@List.app (type.interp A))
+               | List_rev A => @List.rev (type.interp A)
+               | List_fold_right A B => curry3_1 (@List.fold_right (type.interp A) (type.interp B))
+               | List_update_nth T => curry3 (@update_nth (type.interp T))
+               | List_nth_default T => curry3 (@List.nth_default (type.interp T))
+               | Z_runtime_mul => curry2 runtime_mul
+               | Z_runtime_add => curry2 runtime_add
+               | Z_add => curry2 Z.add
+               | Z_mul => curry2 Z.mul
+               | Z_pow => curry2 Z.pow
+               | Z_modulo => curry2 Z.modulo
+               | Z_opp => Z.opp
+               | Z_div => curry2 Z.div
+               | Z_eqb => curry2 Z.eqb
+               | Z_of_nat => Z.of_nat
+               end.
 
-        Module List.
-          Notation seq := List_seq.
-          Notation repeat := List_repeat.
-          Notation combine := List_combine.
-          Notation map := List_map.
-          Notation flat_map := List_flat_map.
-          Notation partition := List_partition.
-          Notation app := List_app.
-          Notation rev := List_rev.
-          Notation fold_right := List_fold_right.
-          Notation update_nth := List_update_nth.
-          Notation nth_default := List_nth_default.
-        End List.
+          Ltac reify
+               mkAppIdent
+               term_is_primitive_const
+               term
+               else_tac :=
+            (*let dummy := match goal with _ => idtac "attempting to reify_op" term end in*)
+            lazymatch term with
+            | Nat.succ ?x => mkAppIdent Nat_succ x
+            | S ?x => mkAppIdent Nat_succ x
+            | @Datatypes.nil ?T
+              => let rT := type.reify T in
+                 mkAppIdent (@ident.nil rT) tt
+            | @Datatypes.cons ?T ?x ?xs
+              => let rT := type.reify T in
+                 mkAppIdent (@ident.cons rT) (x, xs)
+            | @Datatypes.fst ?A ?B ?x
+              => let rA := type.reify A in
+                 let rB := type.reify B in
+                 mkAppIdent (@ident.fst rA rB) x
+            | @Datatypes.snd ?A ?B ?x
+              => let rA := type.reify A in
+                 let rB := type.reify B in
+                 mkAppIdent (@ident.snd rA rB) x
+            | @Datatypes.bool_rect (fun _ => ?T) ?Ptrue ?Pfalse ?b
+              => let rT := type.reify T in
+                 mkAppIdent (@ident.bool_rect rT) (Ptrue, Pfalse, b)
+            | @Datatypes.nat_rect (fun _ => ?T) ?P0 (fun (n' : Datatypes.nat) Pn => ?PS) ?n
+              => let rT := type.reify T in
+                 let pat := fresh "pat" in (* fresh for COQBUG(https://github.com/coq/coq/issues/6562) *)
+                 mkAppIdent (@ident.nat_rect rT) (P0,
+                                                  (fun pat : Datatypes.nat * T
+                                                   => let '(n', Pn) := pat in PS),
+                                                  n)
+            | @Datatypes.nat_rect (fun _ => ?T) ?P0 ?PS ?n
+              => let dummy := match goal with _ => fail 1 "nat_rect successor case is not syntactically a function of two arguments:" PS end in
+                 constr:(I : I)
+            | Nat.pred ?x => mkAppIdent ident.pred x
+            | List.seq ?x ?y  => mkAppIdent ident.List_seq (x, y)
+            | @List.repeat ?A ?x ?y
+              => let rA := type.reify A in
+                 mkAppIdent (@ident.List_repeat rA) (x, y)
+            | @LetIn.Let_In ?A (fun _ => ?B) ?x ?f
+              => let rA := type.reify A in
+                 let rB := type.reify B in
+                 mkAppIdent (@ident.Let_In rA rB) (x, f)
+            | @LetIn.Let_In ?A ?B ?x ?f
+              => let dummy := match goal with _ => fail 1 "Let_In contains a dependent type λ as its second argument:" B end in
+                 constr:(I : I)
+            | @combine ?A ?B ?ls1 ?ls2
+              => let rA := type.reify A in
+                 let rB := type.reify B in
+                 mkAppIdent (@ident.List_combine rA rB) (ls1, ls2)
+            | @List.map ?A ?B ?f ?ls
+              => let rA := type.reify A in
+                 let rB := type.reify B in
+                 mkAppIdent (@ident.List_map rA rB) (f, ls)
+            | @List.flat_map ?A ?B ?f ?ls
+              => let rA := type.reify A in
+                 let rB := type.reify B in
+                 mkAppIdent (@ident.List_flat_map rA rB) (f, ls)
+            | @List.partition ?A ?f ?ls
+              => let rA := type.reify A in
+                 mkAppIdent (@ident.List_partition rA) (f, ls)
+            | @List.app ?A ?ls1 ?ls2
+              => let rA := type.reify A in
+                 mkAppIdent (@ident.List_app rA) (ls1, ls2)
+            | @List.rev ?A ?ls
+              => let rA := type.reify A in
+                 mkAppIdent (@ident.List_rev rA) ls
+            | @List.fold_right ?A ?B (fun b a => ?f) ?a0 ?ls
+              => let rA := type.reify A in
+                 let rB := type.reify B in
+                 let pat := fresh "pat" in (* fresh for COQBUG(https://github.com/coq/coq/issues/6562) *)
+                 mkAppIdent (@ident.List_fold_right rA rB) ((fun pat : B * A => let '(b, a) := pat in f), a0, ls)
+            | @List.fold_right ?A ?B ?f ?a0 ?ls
+              => let dummy := match goal with _ => fail 1 "List.fold_right function argument is not syntactically a function of two arguments:" f end in
+                 constr:(I : I)
+            | @update_nth ?T ?n ?f ?ls
+              => let rT := type.reify T in
+                 mkAppIdent (@ident.List_update_nth rT) (n, f, ls)
+            | @List.nth_default ?T ?d ?ls ?n
+              => let rT := type.reify T in
+                 mkAppIdent (@ident.List_nth_default rT) (d, ls, n)
+            | runtime_mul ?x ?y => mkAppIdent ident.Z_runtime_mul (x, y)
+            | runtime_add ?x ?y => mkAppIdent ident.Z_runtime_add (x, y)
+            | Z.add ?x ?y => mkAppIdent ident.Z_add (x, y)
+            | Z.mul ?x ?y => mkAppIdent ident.Z_mul (x, y)
+            | Z.pow ?x ?y => mkAppIdent ident.Z_pow (x, y)
+            | Z.opp ?x => mkAppIdent ident.Z_opp x
+            | Z.div ?x ?y => mkAppIdent ident.Z_div (x, y)
+            | Z.modulo ?x ?y => mkAppIdent ident.Z_modulo (x, y)
+            | Z.eqb ?x ?y => mkAppIdent ident.Z_eqb (x, y)
+            | Z.of_nat ?x => mkAppIdent ident.Z_of_nat x
+            | _
+              => lazymatch term_is_primitive_const with
+                 | true
+                   =>
+                   let assert_const := match goal with
+                                       | _ => require_primitive_const term
+                                       end in
+                   let T := type of term in
+                   let rT := type.reify_primitive T in
+                   mkAppIdent (@ident.primitive rT term) tt
+                 | false => else_tac ()
+                 end
+            end.
 
-        Module Z.
-          Notation runtime_mul := Z_runtime_mul.
-          Notation runtime_add := Z_runtime_add.
-          Notation add := Z_add.
-          Notation mul := Z_mul.
-          Notation pow := Z_pow.
-          Notation opp := Z_opp.
-          Notation div := Z_div.
-          Notation modulo := Z_modulo.
-          Notation eqb := Z_eqb.
-          Notation of_nat := Z_of_nat.
-        End Z.
+          Module List.
+            Notation seq := List_seq.
+            Notation repeat := List_repeat.
+            Notation combine := List_combine.
+            Notation map := List_map.
+            Notation flat_map := List_flat_map.
+            Notation partition := List_partition.
+            Notation app := List_app.
+            Notation rev := List_rev.
+            Notation fold_right := List_fold_right.
+            Notation update_nth := List_update_nth.
+            Notation nth_default := List_nth_default.
+          End List.
 
-        Module Nat.
-          Notation succ := Nat_succ.
-        End Nat.
+          Module Z.
+            Notation runtime_mul := Z_runtime_mul.
+            Notation runtime_add := Z_runtime_add.
+            Notation add := Z_add.
+            Notation mul := Z_mul.
+            Notation pow := Z_pow.
+            Notation opp := Z_opp.
+            Notation div := Z_div.
+            Notation modulo := Z_modulo.
+            Notation eqb := Z_eqb.
+            Notation of_nat := Z_of_nat.
+          End Z.
 
-        Module Export Notations.
-          Notation ident := ident.
+          Module Nat.
+            Notation succ := Nat_succ.
+          End Nat.
+
+          Module Export Notations.
+            Notation ident := ident.
+          End Notations.
+        End ident.
+
+        Module Notations.
+          Include ident.Notations.
+          Notation expr := (@expr ident).
+          Notation Expr := (@Expr ident).
+          Notation interp := (@interp ident (@ident.interp)).
+          Notation Interp := (@Interp ident (@ident.interp)).
+
+          (*Notation "( x , y , .. , z )" := (Pair .. (Pair x%expr y%expr) .. z%expr) : expr_scope.*)
+          Notation "'expr_let' x := A 'in' b" := (AppIdent ident.Let_In (Pair A%expr (Abs (fun x => b%expr)))) : expr_scope.
+          Notation "[ ]" := (AppIdent ident.nil _) : expr_scope.
+          Notation "x :: xs" := (AppIdent ident.cons (Pair x%expr xs%expr)) : expr_scope.
+          Notation "x" := (AppIdent (ident.primitive x) _) (only printing, at level 9) : expr_scope.
+          Notation "ls [[ n ]]"
+            := (AppIdent ident.List.nth_default (_, ls, AppIdent (ident.primitive n%nat) _)%expr)
+               : expr_scope.
+
+          Module Reification.
+            Ltac reify var term := expr.reify ident ident.reify var term.
+            Ltac Reify term := expr.Reify ident ident.reify term.
+            Ltac Reify_rhs _ :=
+              expr.Reify_rhs ident ident.reify ident.interp ().
+          End Reification.
+          Include Reification.
         End Notations.
-      End ident.
+        Include Notations.
+      End for_reification.
 
-      Module Notations.
-        Include ident.Notations.
-        Notation expr := (@expr ident).
-        Notation Expr := (@Expr ident).
-        Notation interp := (@interp ident (@ident.interp)).
-        Notation Interp := (@Interp ident (@ident.interp)).
+      Module Export default.
+        Module ident.
+          Import type.
+          Inductive ident : type -> type -> Set :=
+          | primitive {t : type.primitive} (v : interp t) : ident () t
+          | Let_In {tx tC} : ident (tx * (tx -> tC)) tC
+          | Nat_succ : ident nat nat
+          | nil {t} : ident () (list t)
+          | cons {t} : ident (t * list t) (list t)
+          | fst {A B} : ident (A * B) A
+          | snd {A B} : ident (A * B) B
+          | bool_rect {T} : ident (T * T * bool) T
+          | nat_rect {P} : ident (P * (nat * P -> P) * nat) P
+          | pred : ident nat nat
+          | list_rect {A P} : ident (P * (A * list A * P -> P) * list A) P
+          | List_nth_default {T} : ident (T * list T * nat) T
+          | Z_runtime_mul : ident (Z * Z) Z
+          | Z_runtime_add : ident (Z * Z) Z
+          | Z_add : ident (Z * Z) Z
+          | Z_mul : ident (Z * Z) Z
+          | Z_pow : ident (Z * Z) Z
+          | Z_opp : ident Z Z
+          | Z_div : ident (Z * Z) Z
+          | Z_modulo : ident (Z * Z) Z
+          | Z_eqb : ident (Z * Z) bool
+          | Z_of_nat : ident nat Z.
 
-        Notation Pair x y := (App (App (Ident ident.pair) x) y).
+          Notation curry0 f
+            := (fun 'tt => f).
+          Notation curry2 f
+            := (fun '(a, b) => f a b).
+          Notation curry3 f
+            := (fun '(a, b, c) => f a b c).
+          Notation uncurry2 f
+            := (fun a b => f (a, b)).
+          Notation uncurry3 f
+            := (fun a b c => f (a, b, c)).
+          Notation curry3_23 f
+            := (fun '(a, b, c) => f a (uncurry3 b) c).
+          Notation curry3_2 f
+            := (fun '(a, b, c) => f a (uncurry2 b) c).
 
-        Notation "( x , y , .. , z )" := (Pair .. (Pair x%expr y%expr) .. z%expr) : expr_scope.
-        Notation "'expr_let' x := A 'in' b" := (App (App (Ident ident.Let_In) A%expr) (Abs (fun x => b%expr))) : expr_scope.
-        Notation "[ ]" := (Ident ident.nil) : expr_scope.
-        Notation "x :: xs" := (App (App (Ident ident.cons) x%expr) xs%expr) : expr_scope.
-        Notation "x" := (Ident (ident.primitive x)) (only printing, at level 9) : expr_scope.
-        Notation "ls [[ n ]]"
-          := (App (App (App (Ident ident.List.nth_default) _) ls%expr) (Ident (ident.primitive n%nat)))
-             : expr_scope.
+          Definition interp {s d} (idc : ident s d) : type.interp s -> type.interp d
+            := match idc in ident s d return type.interp s -> type.interp d with
+               | primitive _ v => curry0 v
+               | Let_In tx tC => curry2 (@LetIn.Let_In (type.interp tx) (fun _ => type.interp tC))
+               | Nat_succ => Nat.succ
+               | nil t => curry0 (@Datatypes.nil (type.interp t))
+               | cons t => curry2 (@Datatypes.cons (type.interp t))
+               | fst A B => @Datatypes.fst (type.interp A) (type.interp B)
+               | snd A B => @Datatypes.snd (type.interp A) (type.interp B)
+               | bool_rect T => curry3 (@Datatypes.bool_rect (fun _ => type.interp T))
+               | nat_rect P => curry3_2 (@Datatypes.nat_rect (fun _ => type.interp P))
+               | pred => Nat.pred
+               | list_rect A P => curry3_23 (@Datatypes.list_rect (type.interp A) (fun _ => type.interp P))
+               | List_nth_default T => curry3 (@List.nth_default (type.interp T))
+               | Z_runtime_mul => curry2 runtime_mul
+               | Z_runtime_add => curry2 runtime_add
+               | Z_add => curry2 Z.add
+               | Z_mul => curry2 Z.mul
+               | Z_pow => curry2 Z.pow
+               | Z_modulo => curry2 Z.modulo
+               | Z_opp => Z.opp
+               | Z_div => curry2 Z.div
+               | Z_eqb => curry2 Z.eqb
+               | Z_of_nat => Z.of_nat
+               end.
 
-        Module Reification.
+          Ltac reify
+               mkAppIdent
+               term_is_primitive_const
+               term
+               else_tac :=
+            (*let dummy := match goal with _ => idtac "attempting to reify_op" term end in*)
+            lazymatch term with
+            | Nat.succ ?x => mkAppIdent Nat_succ x
+            | S ?x => mkAppIdent Nat_succ x
+            | @Datatypes.nil ?T
+              => let rT := type.reify T in
+                 mkAppIdent (@ident.nil rT) tt
+            | @Datatypes.cons ?T ?x ?xs
+              => let rT := type.reify T in
+                 mkAppIdent (@ident.cons rT) (x, xs)
+            | @Datatypes.fst ?A ?B ?x
+              => let rA := type.reify A in
+                 let rB := type.reify B in
+                 mkAppIdent (@ident.fst rA rB) x
+            | @Datatypes.snd ?A ?B ?x
+              => let rA := type.reify A in
+                 let rB := type.reify B in
+                 mkAppIdent (@ident.snd rA rB) x
+            | @Datatypes.bool_rect (fun _ => ?T) ?Ptrue ?Pfalse ?b
+              => let rT := type.reify T in
+                 mkAppIdent (@ident.bool_rect rT) (Ptrue, Pfalse, b)
+            | @Datatypes.nat_rect (fun _ => ?T) ?P0 (fun (n' : Datatypes.nat) Pn => ?PS) ?n
+              => let rT := type.reify T in
+                 let pat := fresh "pat" in (* fresh for COQBUG(https://github.com/coq/coq/issues/6562) *)
+                 mkAppIdent (@ident.nat_rect rT) (P0,
+                                                  (fun pat : Datatypes.nat * T
+                                                   => let '(n', Pn) := pat in PS),
+                                                  n)
+            | @Datatypes.nat_rect (fun _ => ?T) ?P0 ?PS ?n
+              => let dummy := match goal with _ => fail 1 "nat_rect successor case is not syntactically a function of two arguments:" PS end in
+                 constr:(I : I)
+            | Nat.pred ?x => mkAppIdent ident.pred x
+            | @LetIn.Let_In ?A (fun _ => ?B) ?x ?f
+              => let rA := type.reify A in
+                 let rB := type.reify B in
+                 mkAppIdent (@ident.Let_In rA rB) (x, f)
+            | @LetIn.Let_In ?A ?B ?x ?f
+              => let dummy := match goal with _ => fail 1 "Let_In contains a dependent type λ as its second argument:" B end in
+                 constr:(I : I)
+            | @Datatypes.list_rect ?A (fun _ => ?B) ?Pnil (fun x xs rec => ?Pcons) ?ls
+              => let rA := type.reify A in
+                 let rB := type.reify B in
+                 let pat := fresh "pat" in (* fresh for COQBUG(https://github.com/coq/coq/issues/6562) *)
+                 let pat' := fresh "pat" in (* fresh for COQBUG(https://github.com/coq/coq/issues/6562) (must also not overlap with [rec], but I think [fresh] handles that correctly, at least) *)
+                 mkAppIdent (@ident.list_rect rA rB)
+                            (Pnil,
+                             (fun pat : A * Datatypes.list A * B
+                              => let '(pat', rec) := pat in
+                                 let '(x, xs) := pat' in
+                                 Pcons),
+                             ls)
+            | @Datatypes.list_rect ?A (fun _ => ?B) ?Pnil ?Pcons ?ls
+              => let dummy := match goal with _ => fail 1 "list_rect cons case is not syntactically a function of three arguments:" Pcons end in
+                 constr:(I : I)
+            | @List.nth_default ?T ?d ?ls ?n
+              => let rT := type.reify T in
+                 mkAppIdent (@ident.List_nth_default rT) (d, ls, n)
+            | runtime_mul ?x ?y => mkAppIdent ident.Z_runtime_mul (x, y)
+            | runtime_add ?x ?y => mkAppIdent ident.Z_runtime_add (x, y)
+            | Z.add ?x ?y => mkAppIdent ident.Z_add (x, y)
+            | Z.mul ?x ?y => mkAppIdent ident.Z_mul (x, y)
+            | Z.pow ?x ?y => mkAppIdent ident.Z_pow (x, y)
+            | Z.opp ?x => mkAppIdent ident.Z_opp x
+            | Z.div ?x ?y => mkAppIdent ident.Z_div (x, y)
+            | Z.modulo ?x ?y => mkAppIdent ident.Z_modulo (x, y)
+            | Z.eqb ?x ?y => mkAppIdent ident.Z_eqb (x, y)
+            | Z.of_nat ?x => mkAppIdent ident.Z_of_nat x
+            | _
+              => lazymatch term_is_primitive_const with
+                 | true
+                   =>
+                   let assert_const := match goal with
+                                       | _ => require_primitive_const term
+                                       end in
+                   let T := type of term in
+                   let rT := type.reify_primitive T in
+                   mkAppIdent (@ident.primitive rT term) tt
+                 | _ => else_tac ()
+                 end
+            end.
+
+          Module List.
+            Notation nth_default := List_nth_default.
+          End List.
+
+          Module Z.
+            Notation runtime_mul := Z_runtime_mul.
+            Notation runtime_add := Z_runtime_add.
+            Notation add := Z_add.
+            Notation mul := Z_mul.
+            Notation pow := Z_pow.
+            Notation opp := Z_opp.
+            Notation div := Z_div.
+            Notation modulo := Z_modulo.
+            Notation eqb := Z_eqb.
+            Notation of_nat := Z_of_nat.
+          End Z.
+
+          Module Nat.
+            Notation succ := Nat_succ.
+          End Nat.
+
+          Module Export Notations.
+            Notation ident := ident.
+          End Notations.
+        End ident.
+
+        Module Notations.
+          Include ident.Notations.
+          Notation expr := (@expr ident).
+          Notation Expr := (@Expr ident).
+          Notation interp := (@interp ident (@ident.interp)).
+          Notation Interp := (@Interp ident (@ident.interp)).
+
+          (*Notation "( x , y , .. , z )" := (Pair .. (Pair x%expr y%expr) .. z%expr) : expr_scope.*)
+          Notation "'expr_let' x := A 'in' b" := (AppIdent ident.Let_In (Pair A%expr (Abs (fun x => b%expr)))) : expr_scope.
+          Notation "[ ]" := (AppIdent ident.nil _) : expr_scope.
+          Notation "x :: xs" := (AppIdent ident.cons (Pair x%expr xs%expr)) : expr_scope.
+          Notation "x" := (AppIdent (ident.primitive x) _) (only printing, at level 9) : expr_scope.
+          Notation "ls [[ n ]]"
+            := (AppIdent ident.List.nth_default (_, ls, AppIdent (ident.primitive n%nat) _)%expr)
+               : expr_scope.
+
           Ltac reify var term := expr.reify ident ident.reify var term.
           Ltac Reify term := expr.Reify ident ident.reify term.
           Ltac Reify_rhs _ :=
             expr.Reify_rhs ident ident.reify ident.interp ().
-        End Reification.
-        Include Reification.
         End Notations.
-      Include Notations.
-    End for_reification.
+        Include Notations.
+      End default.
+    End expr.
 
-    Module Export default.
+    Module canonicalize_list_recursion.
+      Import expr.
+      Import expr.default.
       Module ident.
-        Import type.
-        Inductive ident : type -> Set :=
-        | primitive {t : type.primitive} (v : interp t) : ident t
-        | Let_In {tx tC} : ident (tx -> (tx -> tC) -> tC)
-        | Nat_succ : ident (nat -> nat)
-        | nil {t} : ident (list t)
-        | cons {t} : ident (t -> list t -> list t)
-        | pair {A B} : ident (A -> B -> A * B)
-        | fst {A B} : ident (A * B -> A)
-        | snd {A B} : ident (A * B -> B)
-        | bool_rect {T} : ident (T -> T -> bool -> T)
-        | nat_rect {P} : ident (P -> (nat -> P -> P) -> nat -> P)
-        | pred : ident (nat -> nat)
-        | list_rect {A P} : ident (P -> (A -> list A -> P -> P) -> list A -> P)
-        | List_nth_default {T} : ident (T -> list T -> nat -> T)
-        | Z_runtime_mul : ident (Z -> Z -> Z)
-        | Z_runtime_add : ident (Z -> Z -> Z)
-        | Z_add : ident (Z -> Z -> Z)
-        | Z_mul : ident (Z -> Z -> Z)
-        | Z_pow : ident (Z -> Z -> Z)
-        | Z_opp : ident (Z -> Z)
-        | Z_div : ident (Z -> Z -> Z)
-        | Z_modulo : ident (Z -> Z -> Z)
-        | Z_eqb : ident (Z -> Z -> bool)
-        | Z_of_nat : ident (nat -> Z).
-
-        Definition interp {t} (idc : ident t) : type.interp t
-          := match idc in ident t return type.interp t with
-             | primitive _ v => v
-             | Let_In tx tC => @LetIn.Let_In (type.interp tx) (fun _ => type.interp tC)
-             | Nat_succ => Nat.succ
-             | nil t => @Datatypes.nil (type.interp t)
-             | cons t => @Datatypes.cons (type.interp t)
-             | pair A B => @Datatypes.pair (type.interp A) (type.interp B)
-             | fst A B => @Datatypes.fst (type.interp A) (type.interp B)
-             | snd A B => @Datatypes.snd (type.interp A) (type.interp B)
-             | bool_rect T => @Datatypes.bool_rect (fun _ => type.interp T)
-             | nat_rect P => @Datatypes.nat_rect (fun _ => type.interp P)
-             | pred => Nat.pred
-             | list_rect A P => @Datatypes.list_rect (type.interp A) (fun _ => type.interp P)
-             | List_nth_default T => @nth_default (type.interp T)
-             | Z_runtime_mul => runtime_mul
-             | Z_runtime_add => runtime_add
-             | Z_add => Z.add
-             | Z_mul => Z.mul
-             | Z_pow => Z.pow
-             | Z_modulo => Z.modulo
-             | Z_opp => Z.opp
-             | Z_div => Z.div
-             | Z_eqb => Z.eqb
-             | Z_of_nat => Z.of_nat
-             end.
-
-        Ltac reify term :=
-          (*let dummy := match goal with _ => idtac "attempting to reify_op" term end in*)
+        Local Ltac SmartApp term :=
           lazymatch term with
-          | Nat.succ => ident.Nat_succ
-          | S => ident.Nat_succ
-          | @Datatypes.nil ?T
-            => let rT := type.reify T in
-               constr:(@ident.nil rT)
-          | @Datatypes.cons ?T
-            => let rT := type.reify T in
-               constr:(@ident.cons rT)
-          | @Datatypes.pair ?A ?B
-            => let rA := type.reify A in
-               let rB := type.reify B in
-               constr:(@ident.pair rA rB)
-          | @Datatypes.fst ?A ?B
-            => let rA := type.reify A in
-               let rB := type.reify B in
-               constr:(@ident.fst rA rB)
-          | @Datatypes.snd ?A ?B
-            => let rA := type.reify A in
-               let rB := type.reify B in
-               constr:(@ident.snd rA rB)
-          | @Datatypes.bool_rect (fun _ => ?T)
-            => let rT := type.reify T in
-               constr:(@ident.bool_rect rT)
-          | @Datatypes.nat_rect (fun _ => ?T)
-            => let rT := type.reify T in
-               constr:(@ident.nat_rect rT)
-          | Nat.pred => ident.pred
-          | @LetIn.Let_In ?A (fun _ => ?B)
-            => let rA := type.reify A in
-               let rB := type.reify B in
-               constr:(@ident.Let_In rA rB)
-          | @LetIn.Let_In ?A ?B
-            => let dummy := match goal with _ => fail 1 "Let_In contains a dependent type λ as its second argument:" B end in
+          | Abs (fun x : @expr ?var ?T => ?f)
+            => eval cbv [unexpr] in (fun x : @expr var T => @unexpr ident.ident var _ f)
+          | Abs (fun x : ?T => ?f)
+            => let dummy := match goal with _ => fail 1 "Invalid var type:" T end in
                constr:(I : I)
-          | @Datatypes.list_rect ?A (fun _ => ?B)
-            => let rA := type.reify A in
-               let rB := type.reify B in
-               constr:(@ident.list_rect rA rB)
-          | @nth_default ?T
-            => let rT := type.reify T in
-               constr:(@ident.List_nth_default rT)
-          | runtime_mul => ident.Z_runtime_mul
-          | runtime_add => ident.Z_runtime_add
-          | Z.add => ident.Z_add
-          | Z.mul => ident.Z_mul
-          | Z.pow => ident.Z_pow
-          | Z.opp => ident.Z_opp
-          | Z.div => ident.Z_div
-          | Z.modulo => ident.Z_modulo
-          | Z.eqb => ident.Z_eqb
-          | Z.of_nat => ident.Z_of_nat
-          | _
-            => let assert_const := match goal with
-                                   | _ => require_primitive_const term
-                                   end in
-               let T := type of term in
-               let rT := type.reify_primitive T in
-               constr:(@ident.primitive rT term)
           end.
 
-        Module List.
-          Notation nth_default := List_nth_default.
-        End List.
-
-        Module Z.
-          Notation runtime_mul := Z_runtime_mul.
-          Notation runtime_add := Z_runtime_add.
-          Notation add := Z_add.
-          Notation mul := Z_mul.
-          Notation pow := Z_pow.
-          Notation opp := Z_opp.
-          Notation div := Z_div.
-          Notation modulo := Z_modulo.
-          Notation eqb := Z_eqb.
-          Notation of_nat := Z_of_nat.
-        End Z.
-
-        Module Nat.
-          Notation succ := Nat_succ.
-        End Nat.
-
-        Module Export Notations.
-          Notation ident := ident.
-        End Notations.
-      End ident.
-
-      Module Notations.
-        Include ident.Notations.
-        Notation expr := (@expr ident).
-        Notation Expr := (@Expr ident).
-        Notation interp := (@interp ident (@ident.interp)).
-        Notation Interp := (@Interp ident (@ident.interp)).
-
-        Notation Pair x y := (App (App (Ident ident.pair) x) y).
-
-        Notation "( x , y , .. , z )" := (Pair .. (Pair x%expr y%expr) .. z%expr) : expr_scope.
-        Notation "'expr_let' x := A 'in' b" := (App (App (Ident ident.Let_In) A%expr) (Abs (fun x => b%expr))) : expr_scope.
-        Notation "[ ]" := (Ident ident.nil) : expr_scope.
-        Notation "x :: xs" := (App (App (Ident ident.cons) x%expr) xs%expr) : expr_scope.
-        Notation "x" := (Ident (ident.primitive x)) (only printing, at level 9) : expr_scope.
-        Notation "ls [[ n ]]"
-          := (App (App (App (Ident ident.List.nth_default) _) ls%expr) (Ident (ident.primitive n%nat)))
-             : expr_scope.
-
-        Ltac reify var term := expr.reify ident ident.reify var term.
-        Ltac Reify term := expr.Reify ident ident.reify term.
-        Ltac Reify_rhs _ :=
-          expr.Reify_rhs ident ident.reify ident.interp ().
-      End Notations.
-      Include Notations.
-    End default.
-  End expr.
-
-  Module canonicalize_list_recursion.
-    Import expr.
-    Import expr.default.
-    Module ident.
-      Definition transfer {var} {t} (idc : for_reification.ident t) : @expr var t
-        := let List_app A :=
-               list_rect
-                 (fun _ => list (type.interp A) -> list (type.interp A))
-                 (fun m => m)
-                 (fun a l1 app_l1 m => a :: app_l1 m) in
-           match idc with
-           | for_reification.ident.Let_In tx tC
-             => Ident ident.Let_In
-           | for_reification.ident.Nat_succ
-             => Ident ident.Nat_succ
-           | for_reification.ident.nil t
-             => Ident ident.nil
-           | for_reification.ident.cons t
-             => Ident ident.cons
-           | for_reification.ident.pair A B
-             => Ident ident.pair
-           | for_reification.ident.fst A B
-             => Ident ident.fst
-           | for_reification.ident.snd A B
-             => Ident ident.snd
-           | for_reification.ident.bool_rect T
-             => Ident ident.bool_rect
-           | for_reification.ident.nat_rect P
-             => Ident ident.nat_rect
-           | for_reification.ident.pred
-             => Ident ident.pred
-           | for_reification.ident.primitive t v
-             => Ident (ident.primitive v)
-           | for_reification.ident.Z_runtime_mul
-             => Ident ident.Z.runtime_mul
-           | for_reification.ident.Z_runtime_add
-             => Ident ident.Z.runtime_add
-           | for_reification.ident.Z_add
-             => Ident ident.Z.add
-           | for_reification.ident.Z_mul
-             => Ident ident.Z.mul
-           | for_reification.ident.Z_pow
-             => Ident ident.Z.pow
-           | for_reification.ident.Z_opp
-             => Ident ident.Z.opp
-           | for_reification.ident.Z_div
-             => Ident ident.Z.div
-           | for_reification.ident.Z_modulo
-             => Ident ident.Z.modulo
-           | for_reification.ident.Z_eqb
-             => Ident ident.Z.eqb
-           | for_reification.ident.Z_of_nat
-             => Ident ident.Z.of_nat
-           | for_reification.ident.List_seq
-             => ltac:(
-                  let v := reify
-                             var
-                             (fun start len : nat
-                              => nat_rect
-                                   (fun _ => nat -> list nat)
-                                   (fun _ => nil)
-                                   (fun len seq_len start => cons start (seq_len (S start)))
-                                   len start)
-                  in exact v)
-           | for_reification.ident.List_repeat A
-             => ltac:(
-                  let v := reify
-                             var
-                             (fun (x : type.interp A)
-                              => nat_rect
-                                   (fun _ => list (type.interp A))
-                                   nil
-                                   (fun k repeat_k => cons x repeat_k)) in
-                  exact v)
-           | for_reification.ident.List_combine A B
-             => ltac:(
-                  let v := reify
-                             var
-                             (list_rect
-                                (fun _ => list (type.interp B) -> list (type.interp A * type.interp B))
-                                (fun l' => nil)
-                                (fun x tl combine_tl
-                                 => list_rect
-                                      (fun _ => list (type.interp A * type.interp B))
-                                      nil
-                                      (fun y tl' REIFICATION_STACK_OVERFLOWS_IF_THIS_IS_NAMED_UNDERSCORE (* CODBUG(https://github.com/coq/coq/issues/5448) *)
-                                       => (x, y) :: combine_tl tl'))) in
-                  exact v)
-           | for_reification.ident.List_map A B
-             => ltac:(
-                  let v := reify
-                             var
-                             (fun f : type.interp A -> type.interp B
-                              => list_rect
-                                   (fun _ => list (type.interp B))
-                                   nil
-                                   (fun a t map_t => f a :: map_t)) in
-                  exact v)
-           | for_reification.ident.List_flat_map A B
-             => ltac:(
-                  let List_app := (eval cbv [List_app] in (List_app B)) in
-                  let v := reify
-                             var
-                             (fun f : type.interp A -> list (type.interp B)
-                              => list_rect
-                                   (fun _ => list (type.interp B))
-                                   nil
-                                   (fun x t flat_map_t => List_app (f x) flat_map_t)) in
-                  exact v)
-           | for_reification.ident.List_partition A
-             => ltac:(
-                  let v := reify
-                             var
-                             (fun f : type.interp A -> bool
-                              => list_rect
-                                   (fun _ => list (type.interp A) * list (type.interp A))%type
-                                   (nil, nil)
-                                   (fun x tl partition_tl
-                                    => let g := fst partition_tl in
-                                       let d := snd partition_tl in
-                                       if f x then (x :: g, d) else (g, x :: d))) in
-                  exact v)
-           | for_reification.ident.List_app A
-             => ltac:(
-                  let List_app := (eval cbv [List_app] in (List_app A)) in
-                  let v := reify var List_app in
-                  exact v)
-           | for_reification.ident.List_rev A
-             => ltac:(
-                  let List_app := (eval cbv [List_app] in (List_app A)) in
-                  let v := reify
-                             var
-                             (list_rect
-                                (fun _ => list (type.interp A))
-                                nil
-                                (fun x l' rev_l' => List_app rev_l' [x])) in
-                  exact v)
-           | for_reification.ident.List_fold_right A B
-             => ltac:(
-                  let v := reify
-                             var
-                             (fun (f : type.interp B -> type.interp A -> type.interp A) (a0 : type.interp A)
-                              => list_rect
-                                   (fun _ => type.interp A)
-                                   a0
-                                   (fun b t fold_right_t => f b fold_right_t)) in
-                  exact v)
-           | for_reification.ident.List_update_nth T
-             => ltac:(
-                  let v := reify
-                             var
-                             (fun (n : nat) (f : type.interp T -> type.interp T)
-                              => nat_rect
-                                   (fun _ => list (type.interp T) -> list (type.interp T))
-                                   (list_rect
-                                      (fun _ => list (type.interp T))
-                                      nil
-                                      (fun x' xs' __ => f x' :: xs'))
-                                   (fun n' update_nth_n'
-                                    => list_rect
-                                         (fun _ => list (type.interp T))
-                                         nil
-                                         (fun x' xs' __ => x' :: update_nth_n' xs'))
-                                   n) in
-                  exact v)
-           | for_reification.ident.List_nth_default T
-             => Ident ident.List_nth_default
-           (*ltac:(
+        Definition transfer {var} {s d} (idc : for_reification.ident s d) : @expr var s -> @expr var d
+          := let List_app A :=
+                 list_rect
+                   (fun _ => list (type.interp A) -> list (type.interp A))
+                   (fun m => m)
+                   (fun a l1 app_l1 m => a :: app_l1 m) in
+             match idc in for_reification.ident s d return @expr var s -> @expr var d with
+             | for_reification.ident.Let_In tx tC
+               => AppIdent ident.Let_In
+             | for_reification.ident.Nat_succ
+               => AppIdent ident.Nat_succ
+             | for_reification.ident.nil t
+               => AppIdent ident.nil
+             | for_reification.ident.cons t
+               => AppIdent ident.cons
+             | for_reification.ident.fst A B
+               => AppIdent ident.fst
+             | for_reification.ident.snd A B
+               => AppIdent ident.snd
+             | for_reification.ident.bool_rect T
+               => AppIdent ident.bool_rect
+             | for_reification.ident.nat_rect P
+               => AppIdent ident.nat_rect
+             | for_reification.ident.pred
+               => AppIdent ident.pred
+             | for_reification.ident.primitive t v
+               => AppIdent (ident.primitive v)
+             | for_reification.ident.Z_runtime_mul
+               => AppIdent ident.Z.runtime_mul
+             | for_reification.ident.Z_runtime_add
+               => AppIdent ident.Z.runtime_add
+             | for_reification.ident.Z_add
+               => AppIdent ident.Z.add
+             | for_reification.ident.Z_mul
+               => AppIdent ident.Z.mul
+             | for_reification.ident.Z_pow
+               => AppIdent ident.Z.pow
+             | for_reification.ident.Z_opp
+               => AppIdent ident.Z.opp
+             | for_reification.ident.Z_div
+               => AppIdent ident.Z.div
+             | for_reification.ident.Z_modulo
+               => AppIdent ident.Z.modulo
+             | for_reification.ident.Z_eqb
+               => AppIdent ident.Z.eqb
+             | for_reification.ident.Z_of_nat
+               => AppIdent ident.Z.of_nat
+             | for_reification.ident.List_seq
+               => ltac:(
+                    let v
+                        :=
+                        reify
+                          (@expr var)
+                          (fun start_len : nat * nat
+                           => nat_rect
+                                (fun _ => nat -> list nat)
+                                (fun _ => nil)
+                                (fun len seq_len start => cons start (seq_len (S start)))
+                                (snd start_len) (fst start_len)) in
+                    let v := SmartApp v in exact v)
+             | for_reification.ident.List_repeat A
+               => ltac:(
+                    let v := reify
+                               (@expr var)
+                               (fun (xn : type.interp A * nat)
+                                => nat_rect
+                                     (fun _ => list (type.interp A))
+                                     nil
+                                     (fun k repeat_k => cons (fst xn) repeat_k)
+                                     (snd xn)) in
+                    let v := SmartApp v in exact v)
+             | for_reification.ident.List_combine A B
+               => ltac:(
+                    let v := reify
+                               (@expr var)
+                               (fun '((ls1, ls2) : list (type.interp A) * list (type.interp B))
+                                => list_rect
+                                     (fun _ => list (type.interp B) -> list (type.interp A * type.interp B))
+                                     (fun l' => nil)
+                                     (fun x tl combine_tl rest
+                                      => list_rect
+                                           (fun _ => list (type.interp A * type.interp B))
+                                           nil
+                                           (fun y tl' _
+                                            => (x, y) :: combine_tl tl')
+                                           rest)
+                                     ls1
+                                     ls2) in
+                    let v := SmartApp v in exact v)
+             | for_reification.ident.List_map A B
+               => ltac:(
+                    let v := reify
+                               (@expr var)
+                               (fun '((f, ls) : (type.interp A -> type.interp B) * Datatypes.list (type.interp A))
+                                => list_rect
+                                     (fun _ => list (type.interp B))
+                                     nil
+                                     (fun a t map_t => f a :: map_t)
+                                     ls) in
+                    let v := SmartApp v in exact v)
+             | for_reification.ident.List_flat_map A B
+               => ltac:(
+                    let List_app := (eval cbv [List_app] in (List_app B)) in
+                    let v := reify
+                               (@expr var)
+                               (fun '((f, ls) : (type.interp A -> list (type.interp B)) * list (type.interp A))
+                                => list_rect
+                                     (fun _ => list (type.interp B))
+                                     nil
+                                     (fun x t flat_map_t => List_app (f x) flat_map_t)
+                                     ls) in
+                    let v := SmartApp v in exact v)
+             | for_reification.ident.List_partition A
+               => ltac:(
+                    let v := reify
+                               (@expr var)
+                               (fun '((f, ls) : (type.interp A -> bool) * list (type.interp A))
+                                => list_rect
+                                     (fun _ => list (type.interp A) * list (type.interp A))%type
+                                     (nil, nil)
+                                     (fun x tl partition_tl
+                                      => let g := fst partition_tl in
+                                         let d := snd partition_tl in
+                                         if f x then (x :: g, d) else (g, x :: d))
+                                     ls) in
+                    let v := SmartApp v in exact v)
+             | for_reification.ident.List_app A
+               => ltac:(
+                    let List_app := (eval cbv [List_app] in (List_app A)) in
+                    let v := reify (@expr var) (fun '(ls1, ls2) => List_app ls1 ls2) in
+                    let v := SmartApp v in exact v)
+             | for_reification.ident.List_rev A
+               => ltac:(
+                    let List_app := (eval cbv [List_app] in (List_app A)) in
+                    let v := reify
+                               (@expr var)
+                               (fun ls
+                                => list_rect
+                                     (fun _ => list (type.interp A))
+                                     nil
+                                     (fun x l' rev_l' => List_app rev_l' [x])
+                                     ls) in
+                    let v := SmartApp v in exact v)
+             | for_reification.ident.List_fold_right A B
+               => ltac:(
+                    let v := reify
+                               (@expr var)
+                               (fun '((f, a0, ls)
+                                      : (type.interp B * type.interp A -> type.interp A) * type.interp A * list (type.interp B))
+                                => list_rect
+                                     (fun _ => type.interp A)
+                                     a0
+                                     (fun b t fold_right_t => f (b, fold_right_t))
+                                     ls) in
+                    let v := SmartApp v in exact v)
+             | for_reification.ident.List_update_nth T
+               => ltac:(
+                    let v := reify
+                               (@expr var)
+                               (fun '((n, f, ls) : nat * (type.interp T -> type.interp T) * list (type.interp T))
+                                => nat_rect
+                                     (fun _ => list (type.interp T) -> list (type.interp T))
+                                     (fun ls
+                                      => list_rect
+                                           (fun _ => list (type.interp T))
+                                           nil
+                                           (fun x' xs' __ => f x' :: xs')
+                                           ls)
+                                     (fun n' update_nth_n' ls
+                                      => list_rect
+                                           (fun _ => list (type.interp T))
+                                           nil
+                                           (fun x' xs' __ => x' :: update_nth_n' xs')
+                                           ls)
+                                     n
+                                     ls) in
+                    let v := SmartApp v in exact v)
+             | for_reification.ident.List_nth_default T
+               => AppIdent ident.List_nth_default
+             (*ltac:(
                   let v := reify
                              var
                              (fun (default : type.interp T) (l : list (type.interp T)) (n : nat)
@@ -1139,252 +1294,578 @@ Module Compilers.
                                    n
                                    l) in
                   exact v)*)
-           end%expr.
-    End ident.
+             end%expr.
+      End ident.
 
-    Module expr.
-      Section with_var.
-        Context {var : type -> Type}.
+      Module expr.
+        Section with_var.
+          Context {var : type -> Type}.
 
-        Fixpoint transfer {t} (e : @for_reification.Notations.expr var t)
-          : @expr var t
-          := match e  with
-             | Var t v => Var v
-             | Ident t idc => @ident.transfer var t idc
-             | App s d f x => App (@transfer _ f) (@transfer _ x)
-             | Abs s d f => Abs (fun x => @transfer d (f x))
-             end.
-      End with_var.
+          Fixpoint transfer {t} (e : @for_reification.Notations.expr var t)
+            : @expr var t
+            := match e  with
+               | Var t v => Var v
+               | TT => TT
+               | Pair A B a b => Pair (@transfer A a) (@transfer B b)
+               | AppIdent s d idc args => @ident.transfer var s d idc (@transfer _ args)
+               | App s d f x => App (@transfer _ f) (@transfer _ x)
+               | Abs s d f => Abs (fun x => @transfer d (f x))
+               end.
+        End with_var.
 
-      Definition Transfer {t} (e : for_reification.Notations.Expr t) : Expr t
-        := fun var => transfer (e _).
-    End expr.
-  End canonicalize_list_recursion.
-  Notation canonicalize_list_recursion := canonicalize_list_recursion.expr.Transfer.
-  Import expr.
-  Import expr.default.
+        Definition Transfer {t} (e : for_reification.Notations.Expr t) : Expr t
+          := fun var => transfer (e _).
+      End expr.
+    End canonicalize_list_recursion.
+    Notation canonicalize_list_recursion := canonicalize_list_recursion.expr.Transfer.
+    Export expr.
+    Export expr.default.
+  End Uncurried.
 
   Module CPS.
+    Import Uncurried.
+    Module Import Output.
+      Module type.
+        Import Compilers.type.
+        Inductive type := type_primitive (_:primitive) | prod (A B : type) | continuation (A : type) | list (A : type).
+        Module Export Coercions.
+          Global Coercion type_primitive : primitive >-> type.
+        End Coercions.
+
+        Module Export Notations.
+          Export Coercions.
+          Delimit Scope cpstype_scope with cpstype.
+          Bind Scope cpstype_scope with type.
+          Notation "()" := unit : cpstype_scope.
+          Notation "A * B" := (prod A B) : cpstype_scope.
+          Notation "A --->" := (continuation A) : cpstype_scope.
+          Notation type := type.
+        End Notations.
+
+        Section interp.
+          Context (R : Type).
+          Fixpoint interp (t : type)
+            := match t return Type with
+               | type_primitive t => Compilers.type.interp t
+               | prod A B => interp A * interp B
+               | continuation A => interp A -> R
+               | list A => Datatypes.list (interp A)
+               end%type.
+        End interp.
+      End type.
+      Export type.Notations.
+
+      Module expr.
+        Section expr.
+          Context {ident : type -> Type} {var : type -> Type} {R : type}.
+
+          Inductive expr :=
+          | Halt (v : var R)
+          | App {A} (f : var (A --->)) (x : var A)
+          | Bind {A} (x : primop A) (f : var A -> expr)
+          with
+          primop : type -> Type :=
+          | Var {t} (v : var t) : primop t
+          | Abs {t} (f : var t -> expr) : primop (t --->)
+          | Pair {A B} (x : var A) (y : var B) : primop (A * B)
+          | Fst {A B} (x : var (A * B)) : primop A
+          | Snd {A B} (x : var (A * B)) : primop B
+          | TT : primop ()
+          | Ident {t} (idc : ident t) : primop t.
+        End expr.
+        Global Arguments expr {ident var} R.
+        Global Arguments primop {ident var} R _.
+
+        Definition Expr {ident : type -> Type} R := forall var, @expr ident var R.
+
+        Section with_ident.
+          Context {ident : type -> Type}
+                  (r : type)
+                  (R : Type)
+                  (interp_ident
+                   : forall t, ident t -> type.interp R t).
+
+          Fixpoint interp (e : @expr ident (type.interp R) r) (k : type.interp R r -> R)
+                   {struct e}
+            : R
+            := match e with
+               | Halt v => k v
+               | App A f x => f x
+               | Bind A x f => interp (f (@interp_primop _ x k)) k
+               end
+          with interp_primop {t} (e : @primop ident (type.interp R) r t) (k : type.interp R r -> R)
+                             {struct e}
+               : type.interp R t
+               := match e with
+                  | Var t v => v
+                  | Abs t f => fun x : type.interp _ t => interp (f x) k
+                  | Pair A B x y => (x, y)
+                  | Fst A B x => fst x
+                  | Snd A B x => snd x
+                  | TT => tt
+                  | Ident t idc => interp_ident t idc
+                  end.
+
+          Definition Interp (e : Expr r) (k : type.interp R r -> R) : R := interp (e _) k.
+        End with_ident.
+
+        Module Export Notations.
+          Delimit Scope cpsexpr_scope with cpsexpr.
+          Bind Scope cpsexpr_scope with expr.
+          Bind Scope cpsexpr_scope with primop.
+
+          Infix "@" := App : cpsexpr_scope.
+          Notation "v <- x ; f" := (Bind x (fun v => f)) : cpsexpr_scope.
+          Notation "'λ'  x .. y , t" := (Abs (fun x => .. (Abs (fun y => t%cpsexpr)) ..)) : cpsexpr_scope.
+          Notation "( x , y , .. , z )" := (Pair .. (Pair x%cpsexpr y%cpsexpr) .. z%cpsexpr) : cpsexpr_scope.
+        Notation "( )" := TT : cpsexpr_scope.
+        Notation "()" := TT : cpsexpr_scope.
+        End Notations.
+      End expr.
+      Export expr.Notations.
+    End Output.
+
     Module type.
-      Import Compilers.type.
       Section translate.
-        Context (R : type).
-        Fixpoint translate (t : type) : type
+        Fixpoint translate (t : Compilers.type.type) : type
           := match t with
-             | A * B => translate A * translate B
-             | s -> d => translate s -> (translate d -> R) -> R
-             | list A => list (translate A)
-             | type_primitive _ as t
+             | A * B => (translate A * translate B)%cpstype
+             | s -> d => (translate s * (translate d --->) --->)%cpstype
+             | Compilers.type.list A => type.list (translate A)
+             | Compilers.type.type_primitive t
                => t
              end%ctype.
+        Fixpoint untranslate (R : Compilers.type.type) (t : type)
+          : Compilers.type.type
+          := match t with
+             | type.type_primitive t => t
+             | A * B => (untranslate R A * untranslate R B)%ctype
+             | (t --->)
+               => (untranslate R t -> R)%ctype
+             | type.list A => Compilers.type.list (untranslate R A)
+             end%cpstype.
       End translate.
     End type.
 
-    Module ident.
-      Section with_var.
-        Context {var : type -> Type}.
-        Let Ident' := @Ident ident var.
-        Local Coercion Ident' : ident >-> expr.
-
-        Definition translate {t} {R}
-                 (idc : ident t)
-                 (k : @expr var (type.translate R t) -> @expr var R)
-          : @expr var R
-          := match idc in ident.ident t return (expr (type.translate R t) -> expr R) -> expr R with
-             | ident.primitive _ _ as idc
-               => fun k => k idc
-             | ident.nil t
-               => fun k => k (@ident.nil (type.translate R t))
-             | ident.Let_In tx tC as idc
-               => fun k
-                  => k (λ (x : var (type.translate R tx))
-                          (xk :
-                             (* ignore this line; it's to work around lack of fixpoint refolding in type inference *) var (((type.translate _ tx -> ((type.translate _ tC -> R) -> R)) -> ((type.translate _ tC -> R) -> R)) -> R)) ,
-                        Var xk @ (λ f fk,
-                                  ident.Let_In
-                                    @ Var x
-                                    @ (λ x, Var f @ Var x @ Var fk)))
-             | ident.Nat_succ as idc
-             | ident.pred as idc
-             | ident.Z_opp as idc
-             | ident.Z_of_nat as idc
-               => fun k
-                  => k (λ x k, Var k @ (idc @ Var x))
-             | ident.cons t as idc
-               => fun k
-                  => k (λ (x : var (type.translate R t))
-                          (xk :
-                             (* ignore this line; it's to work around lack of fixpoint refolding in type inference *) var ((type.list (type.translate _ t) -> ((type.list (type.translate _ t) -> R) -> R)) -> R)),
-                        Var xk @ (λ xs k,
-                                  Var k @ (ident.cons @ Var x @ Var xs)))
-             | ident.pair A B
-               => fun k
-                  => k (λ (x : var (type.translate R A))
-                          (xk :
-                             (* ignore this line; it's to work around lack of fixpoint refolding in type inference *) var ((type.translate _ B -> ((type.translate _ A * type.translate _ B -> R) -> R)) -> R)),
-                        Var xk @ (λ y k,
-                                  Var k @ (Var x, Var y)))
-             | ident.fst A B
-               => fun k
-                  => k (λ (x : var (type.translate R A * type.translate R B))
-                          (k : var (type.translate _ A -> R)),
-                        Var k @ (ident.fst @ Var x))
-             | ident.snd A B
-               => fun k
-                  => k (λ (x : var (type.translate R A * type.translate R B))
-                          (k : var (type.translate _ B -> R)),
-                        Var k @ (ident.snd @ Var x))
-             | ident.bool_rect T
-               => fun k
-                  => k (λ (true_case : var (type.translate R T))
-                          (k0 :
-                             (* ignore this line; it's to work around lack of fixpoint refolding in type inference *) var ((type.translate R T -> ((type.bool -> (type.translate R T -> R) -> R) -> R) -> R) -> R)),
-                        Var k0 @ (λ false_case k1,
-                                  Var k1 @ (λ b k,
-                                            ident.bool_rect
-                                              @ (Var k @ Var true_case)
-                                              @ (Var k @ Var false_case)
-                                              @ Var b)))
-             | ident.nat_rect P
-               => fun k
-                  => k (λ (O_case : var (type.translate R P))
-                          (k0 :
-                             (* ignore this line; it's to work around lack of fixpoint refolding in type inference *) var (((type.nat -> ((type.translate R P -> (type.translate R P -> R) -> R) -> R) -> R) -> ((type.nat -> (type.translate R P -> R) -> R) -> R) -> R) -> R)),
-                        Var k0 @ (λ S_case k1,
-                                  Var k1 @ (λ n k,
-                                            (@ident.nat_rect ((type.translate R P -> R) -> R))
-                                              @ (λ k, Var k @ Var O_case)
-                                              @ (λ n' rec k,
-                                                 (Var rec)
-                                                   @ (λ rec,
-                                                      (Var S_case)
-                                                        @ (Var n')
-                                                        @ (λ K, Var K @ Var rec @ Var k)))
-                                              @ (Var n)
-                                              @ (Var k))))
-             | ident.list_rect A P
-               => fun k
-                  => k (λ (nil_case : var (type.translate R P))
-                          (k0 :
-                             (* ignore this line; it's to work around lack of fixpoint refolding in type inference *) var (((type.translate R A -> ((type.list (type.translate R A) -> ((type.translate R P -> (type.translate R P -> R) -> R) -> R) -> R) -> R) -> R) -> ((type.list (type.translate R A) -> (type.translate R P -> R) -> R) -> R) -> R) -> R)),
-                        (Var k0)
-                          @ (λ cons_case k1,
-                             (Var k1)
-                               @ (λ ls k,
-                                  (@ident.list_rect _ ((type.translate R P -> R) -> R))
-                                    @ (λ k, Var k @ Var nil_case)
-                                    @ (λ x xs rec k,
-                                       (Var rec)
-                                         @ (λ rec,
-                                            (Var cons_case)
-                                              @ (Var x)
-                                              @ (λ K,
-                                                 (Var K)
-                                                   @ (Var xs)
-                                                   @ (λ K, Var K @ Var rec @ Var k))))
-                                    @ (Var ls)
-                                    @ (Var k))))
-             | ident.List_nth_default A
-               => fun k
-                  => k (λ (default : var (type.translate R A))
-                          (k0 :
-                             (* ignore this line; it's to work around lack of fixpoint refolding in type inference *) var ((type.list (type.translate R A) -> ((type.nat -> (type.translate R A -> R) -> R) -> R) -> R) -> R)),
-                        (Var k0)
-                          @ (λ ls k1,
-                             (Var k1)
-                               @ (λ n k,
-                                  Var k @ (ident.List.nth_default @ Var default @ Var ls @ Var n))))
-             | ident.Z_runtime_mul as idc
-             | ident.Z_runtime_add as idc
-             | ident.Z_add as idc
-             | ident.Z_mul as idc
-             | ident.Z_pow as idc
-             | ident.Z_div as idc
-             | ident.Z_modulo as idc
-             | ident.Z_eqb as idc
-               => fun k
-                  => k (λ x xk,
-                        (Var xk)
-                          @ (λ y yk,
-                             (Var yk @ (idc @ Var x @ Var y))))
-             end%expr k.
-      End with_var.
-    End ident.
-
     Module expr.
-      Section with_var.
-        Context {var : type -> Type}.
-        Notation var' R := (fun t => var (type.translate R t)).
-        Section with_R.
-          Context {R : type}.
+      Import Output.expr.
+      Import Output.expr.Notations.
+      Import Compilers.type.
+      Import Compilers.Uncurried.expr.
+      Section with_ident.
+        Context {ident : Output.type.type -> Type}
+                {ident' : type -> type -> Type}
+                {var : Output.type.type -> Type}
+                (translate_ident : forall s d, ident' s d -> ident (type.translate (s -> d))).
+        Notation var' := (fun t => var (type.translate t)).
+        Local Notation oexpr := (@Output.expr.expr ident var).
 
-          Fixpoint translate {t}
-                   (e : @expr (var' R) t)
-                   (k : @expr var (type.translate R t) -> @expr var R)
-                   {struct e}
-            : @expr var R
-            := match e in expr.expr t return (expr (type.translate R t) -> expr R) -> expr R with
-               | Var t v
-                 => fun k => k (Var v)
-               | Ident t idc => ident.translate idc
-               | App s d f x
-                 => fun k
-                    => @translate
-                         _ f
-                         (fun fv
-                          => @translate
-                               _ x
-                               (fun xv
-                                => App (App fv xv) (Abs (fun v => k (Var v)))))
-               | Abs s d f
-                 => fun k
-                    => k (Abs (fun (x : var (type.translate R s))
-                               => Abs (fun (k : var (type.translate _ _ -> _))
-                                       => @translate
-                                            _ (f x)
-                                            (fun v => App (Var k) v))))
-               end k.
+        Section splice.
+          Context {r1 r2 : Output.type.type}.
+          Fixpoint splice  (e1 : oexpr r1) (e2 : var r1 -> oexpr r2)
+                   {struct e1}
+            : oexpr r2
+            := match e1 with
+               | Halt v => e2 v
+               | f @ x => f @ x
+               | Bind A x f => v <- @splice_primop _ x e2; @splice (f v) e2
+               end%cpsexpr
+          with
+          splice_primop {t} (f : @primop ident var r1 t) (e2 : var r1 -> oexpr r2)
+                        {struct f}
+          : @primop ident var r2 t
+          := match f with
+             | Output.expr.Var t v => Output.expr.Var v
+             | Output.expr.Pair A B x y as e => Output.expr.Pair x y
+             | Output.expr.Fst A B x => Output.expr.Fst x
+             | Output.expr.Snd A B x => Output.expr.Snd x
+             | Output.expr.TT => Output.expr.TT
+             | Output.expr.Ident t idc => Output.expr.Ident idc
+             | Output.expr.Abs t f
+               => Output.expr.Abs (fun x => @splice (f x) e2)
+             end.
+        End splice.
 
-          Fixpoint collect_translation_function_types t
-            := match t return Type with
-               | type.arrow s d
-                 => collect_translation_function_types d
-                    * (var s -> var (type.translate R s))
-               | _ => unit
-               end%type.
-        End with_R.
+        Local Notation "x <-- e1 ; e2" := (splice e1 (fun x => e2%cpsexpr)) : cpsexpr_scope.
 
-        Fixpoint translate_under_binders {t}
-                 (R:=type.final_codomain t)
-                 (e : @expr (var' R) t)
-                 (k_vars : @collect_translation_function_types (type.final_codomain t) t)
-                 (k : @expr var (type.translate R (type.final_codomain t)) -> @expr var R)
-                 {struct t}
-          : @expr var t
-          := match t return @expr (var' (type.final_codomain t)) t -> (collect_translation_function_types t) -> (expr (type.translate _ (type.final_codomain t)) -> expr (type.final_codomain t)) -> expr t with
-             | type.arrow s d
-               => fun e '((k_vars, ks) : collect_translation_function_types d * _) k
-                  => Abs (fun x : var s
-                          => @translate_under_binders d (e @ Var (ks x))%expr k_vars k)
-             | t
-               => fun e _ k
-                  => @translate (type.final_codomain t) t e k
-             end e k_vars k.
-      End with_var.
+        Fixpoint translate {t}
+                 (e : @Compilers.Uncurried.expr.expr ident' var' t)
+          : @Output.expr.expr ident var (type.translate t)
+          := match e with
+             | Var t v => Halt v
+             | TT => x <- () ; Halt x
+             | AppIdent s d idc args
+               => (args' <-- @translate _ args;
+                     k <- Output.expr.Abs (fun r => Halt r);
+                     p <- (args', k);
+                     f <- Output.expr.Ident (translate_ident s d idc);
+                     f @ p)
+             | Pair A B a b
+               => (a' <-- @translate _ a;
+                     b' <-- @translate _ b;
+                     p <- (a', b');
+                     Halt p)
+             | App s d e1 e2
+               => (f <-- @translate _ e1;
+                     x <-- @translate _ e2;
+                     k <- Output.expr.Abs (fun r => Halt r);
+                     p <- (x, k);
+                     f @ p)
+             | Abs s d f
+               => f <- (Output.expr.Abs
+                          (fun p
+                           => x <- Fst p;
+                                k <- Snd p;
+                                r <-- @translate _ (f x);
+                                k @ r));
+                    Halt f
+             end%cpsexpr.
+      End with_ident.
 
-      Definition Translate {R t} (e : Expr t) (k : forall var, @expr var (type.translate R t) -> @expr var R)
-        : Expr R
-        := fun var => @translate var R t (e _) (k _).
+      Definition Translate
+                 {ident : Output.type.type -> Type}
+                 {ident' : type -> type -> Type}
+                 (translate_ident : forall s d, ident' s d -> ident (type.translate (s -> d)))
+                 {t} (e : @Compilers.Uncurried.expr.Expr ident' t)
+        : @Output.expr.Expr ident (type.translate t)
+        := fun var => translate translate_ident (e _).
 
-      Definition TranslateUnderBinders {t} (e : Expr t)
-                 (k : forall var,
-                     @collect_translation_function_types var (type.final_codomain t) t
-                     * (@expr var (type.translate (type.final_codomain t) (type.final_codomain t)) -> @expr var (type.final_codomain t)))
-        : Expr t
-        := fun var => @translate_under_binders var t (e _) (fst (k _)) (snd (k _)).
+      Section call_with_cont.
+        Context {ident' : Output.type.type -> Type}
+                {ident : type -> type -> Type}
+                {var : type -> Type}
+                {r : Output.type.type}
+                {R : type}.
+        Notation ucexpr := (@Compilers.Uncurried.expr.expr ident var).
+        Notation ucexprut t := (ucexpr (type.untranslate R t)) (only parsing).
+        Notation var' := (fun t => ucexprut t).
+        Context (untranslate_ident : forall t, ident' t -> ucexprut t)
+                (ifst : forall A B, ident (A * B)%ctype A)
+                (isnd : forall A B, ident (A * B)%ctype B).
+
+        Fixpoint call_with_continuation
+                 (e : @Output.expr.expr ident' var' r)
+                 (k : ucexprut r -> ucexpr R)
+                 {struct e}
+          : ucexpr R
+          := match e with
+             | Halt v => k v
+             | expr.App A f x
+               => @App _ _ (type.untranslate R A) R
+                       f x
+             | Bind A x f
+               => @call_with_continuation
+                    (f (@call_primop_with_continuation A x k))
+                    k
+             end%expr
+        with
+        call_primop_with_continuation
+          {t}
+          (e : @Output.expr.primop ident' var' r t)
+          (k : ucexprut r -> ucexpr R)
+          {struct e}
+        : ucexprut t
+        := match e in Output.expr.primop _ t return ucexprut t with
+           | expr.Var t v => v
+           | expr.Abs t f => Abs (fun x : var (type.untranslate _ _)
+                                  => @call_with_continuation
+                                       (f (Var x)) k)
+           | expr.Pair A B x y => (x, y)
+           | Fst A B x => ifst (type.untranslate _ A) (type.untranslate _ B)
+                               @@ x
+           | Snd A B x => isnd (type.untranslate _ A) (type.untranslate _ B)
+                               @@ x
+           | expr.TT => TT
+           | Ident t idc => untranslate_ident t idc
+           end%expr.
+      End call_with_cont.
+
+      Definition CallWithContinuation
+                 {ident' : Output.type.type -> Type}
+                 {ident : type -> type -> Type}
+                 {R : type}
+                 (untranslate_ident : forall t, ident' t -> @Compilers.Uncurried.expr.Expr ident (type.untranslate R t))
+                 (ifst : forall A B, ident (A * B)%ctype A)
+                 (isnd : forall A B, ident (A * B)%ctype B)
+                 {t} (e : @Output.expr.Expr ident' t)
+                 (k : forall var, @Uncurried.expr.expr ident var (type.untranslate R t) -> @Uncurried.expr.expr ident var R)
+        : @Compilers.Uncurried.expr.Expr ident R
+        := fun var => call_with_continuation
+                        (fun t idc => untranslate_ident t idc _) ifst isnd (e _) (k _).
     End expr.
+
+    Module ident.
+      Import CPS.Output.type.
+      Inductive ident : type -> Set :=
+      | wrap {s d} (idc : Uncurried.expr.default.ident s d) : ident (type.translate (s -> d)).
+
+      Notation cps_of f
+        := (fun x k => k (f x)).
+      Notation curry0 f
+        := (fun 'tt => f).
+      Notation curry2 f
+        := (fun '(a, b) => f a b).
+      Notation curry3 f
+        := (fun '(a, b, c) => f a b c).
+      Notation uncurry2 f
+        := (fun a b => f (a, b)).
+      Notation uncurry3 f
+        := (fun a b c => f (a, b, c)).
+      Notation curry3_23 f
+        := (fun '(a, b, c) => f a (uncurry3 b) c).
+      Notation curry3_2 f
+        := (fun '(a, b, c) => f a (uncurry2 b) c).
+
+      Definition interp {R} {t} (idc : ident t) : type.interp R t
+        := match idc in ident t return type.interp R t with
+           | wrap s d idc
+             => fun '((x, k) : type.interp R (type.translate s) * (type.interp R (type.translate d) -> R))
+                =>
+                  match idc in Uncurried.expr.default.ident s d return type.interp R (type.translate s) -> (type.interp R (type.translate d) -> R) -> R with
+                  | ident.primitive _ _ as idc
+                  | ident.Nat_succ as idc
+                  | ident.pred as idc
+                  | ident.Z_runtime_mul as idc
+                  | ident.Z_runtime_add as idc
+                  | ident.Z_add as idc
+                  | ident.Z_mul as idc
+                  | ident.Z_pow as idc
+                  | ident.Z_opp as idc
+                  | ident.Z_div as idc
+                  | ident.Z_modulo as idc
+                  | ident.Z_eqb as idc
+                  | ident.Z_of_nat as idc
+                    => cps_of (Uncurried.expr.default.ident.interp idc)
+                  | ident.Let_In tx tC
+                    => fun '((x, f) : (interp R (type.translate tx)
+                                       * (interp R (type.translate tx) * (interp R (type.translate tC) -> R) -> R)))
+                           (k : interp R (type.translate tC) -> R)
+                       => @LetIn.Let_In
+                            (type.interp R (type.translate tx)) (fun _ => R)
+                            x
+                            (fun v => f (v, k))
+                  | ident.nil t
+                    => cps_of (curry0 (@Datatypes.nil (interp R (type.translate t))))
+                  | ident.cons t
+                    => cps_of (curry2 (@Datatypes.cons (interp R (type.translate t))))
+                  | ident.fst A B
+                    => cps_of (@Datatypes.fst (interp R (type.translate A)) (interp R (type.translate B)))
+                  | ident.snd A B
+                    => cps_of (@Datatypes.snd (interp R (type.translate A)) (interp R (type.translate B)))
+                  | ident.bool_rect T
+                    => fun '((tc, fc, b) :
+                               (* ignore this line; it's to work around lack of fixpoint refolding in type inference *) type.interp R (type.translate T) * type.interp R (type.translate T) * bool)
+                           k
+                       => @Datatypes.bool_rect
+                            (fun _ => R)
+                            (k tc)
+                            (k fc)
+                            b
+                  | ident.nat_rect P
+                    => fun '((PO, PS, n) :
+                               (* ignore this line; it's to work around lack of fixpoint refolding in type inference *) interp R (type.translate P) * (nat * interp R (type.translate P) * (interp R (type.translate P) -> R) -> R) * nat)
+                           k
+                       => @Datatypes.nat_rect
+                            (fun _ => (interp R (type.translate P) -> R) -> R)
+                            (fun k => k PO)
+                            (fun n' rec k
+                             => rec (fun rec => PS (n', rec, k)))
+                            n
+                            k
+                  | ident.list_rect A P
+                    => fun '((Pnil, Pcons, ls) :
+                               (* ignore this line; it's to work around lack of fixpoint refolding in type inference *) interp R (type.translate P) * (interp R (type.translate A) * Datatypes.list (interp R (type.translate A)) * interp R (type.translate P) * (interp R (type.translate P) -> R) -> R) * Datatypes.list (interp R (type.translate A)))
+                           k
+                       => @Datatypes.list_rect
+                            (interp R (type.translate A))
+                            (fun _ => (interp R (type.translate P) -> R) -> R)
+                            (fun k => k Pnil)
+                            (fun x xs rec k
+                             => rec (fun rec => Pcons (x, xs, rec, k)))
+                            ls
+                            k
+                  | ident.List_nth_default T
+                    => cps_of (curry3 (@List.nth_default (interp R (type.translate T))))
+                  end x k
+           end.
+
+      Local Notation var_eta x := (ident.fst @@ x, ident.snd @@ x)%core%expr.
+
+      Definition untranslate {R} {t} (idc : ident t)
+        : @Compilers.Uncurried.expr.Expr Uncurried.expr.default.ident (type.untranslate R t)
+        := fun var
+           => match idc in ident t return Compilers.Uncurried.expr.expr (type.untranslate _ t) with
+              | wrap s d idc
+                =>
+                match idc in default.ident s d return Compilers.Uncurried.expr.expr (type.untranslate _ (type.translate (s -> d))) with
+                | ident.primitive t v
+                  => λ (_k :
+                          (* ignore this line; it's to work around lack of fixpoint refolding in type inference *) var (() * (t -> R))%ctype) ,
+                     (ident.snd @@ (Var _k))
+                       @ (ident.primitive v @@ TT)
+                | ident.Let_In tx tC
+                  => λ (xyk :
+                          (* ignore this line; it's to work around lack of fixpoint refolding in type inference *) var (type.untranslate _ (type.translate tx) * (type.untranslate _ (type.translate tx) * (type.untranslate _ (type.translate tC) -> R) -> R) * (type.untranslate _ (type.translate tC) -> R))%ctype) ,
+                     ident.Let_In
+                       @@ (ident.fst @@ (ident.fst @@ (Var xyk)),
+                           (λ (x :
+                                 (* ignore this line; it's to work around lack of fixpoint refolding in type inference *) var (type.untranslate _ (type.translate tx))) ,
+                            (ident.snd @@ (ident.fst @@ (Var xyk)))
+                              @ (Var x, ident.snd @@ Var xyk)))
+                | ident.nat_rect P
+                  => λ (PO_PS_n_k :
+                          (* ignore this line; it's to work around lack of fixpoint refolding in type inference *) var (type.untranslate _ (type.translate P) * (type.nat * type.untranslate _ (type.translate P) * (type.untranslate _ (type.translate P) -> R) -> R) * type.nat * (type.untranslate _ (type.translate P) -> R))%ctype) ,
+                     let (PO_PS_n, k) := var_eta (Var PO_PS_n_k) in
+                     let (PO_PS, n) := var_eta PO_PS_n in
+                     let (PO, PS) := var_eta PO_PS in
+                     ((@ident.nat_rect ((type.untranslate _ (type.translate P) -> R) -> R))
+                        @@ ((λ k , Var k @ PO),
+                            (λ n'rec k ,
+                             let (n', rec) := var_eta (Var n'rec) in
+                             rec @ (λ rec , PS @ (n', Var rec, Var k))),
+                            n))
+                       @ k
+                | ident.list_rect A P
+                  => λ (Pnil_Pcons_ls_k :
+                          (* ignore this line; it's to work around lack of fixpoint refolding in type inference *) var (type.untranslate _ (type.translate P) * (type.untranslate _ (type.translate A) * Compilers.type.list (type.untranslate _ (type.translate A)) * type.untranslate _ (type.translate P) * (type.untranslate _ (type.translate P) -> R) -> R) * Compilers.type.list (type.untranslate _ (type.translate A)) * (type.untranslate _ (type.translate P) -> R))%ctype) ,
+                     let (Pnil_Pcons_ls, k) := var_eta (Var Pnil_Pcons_ls_k) in
+                     let (Pnil_Pcons, ls) := var_eta Pnil_Pcons_ls in
+                     let (Pnil, Pcons) := var_eta Pnil_Pcons in
+                     ((@ident.list_rect
+                         (type.untranslate _ (type.translate A))
+                         ((type.untranslate _ (type.translate P) -> R) -> R))
+                        @@ ((λ k, Var k @ Pnil),
+                            (λ x_xs_rec k,
+                             let (x_xs, rec) := var_eta (Var x_xs_rec) in
+                             let (x, xs) := var_eta x_xs in
+                             rec @ (λ rec , Pcons @ (x, xs, Var rec, Var k))),
+                            ls))
+                       @ k
+                | ident.List_nth_default T
+                  => λ (xyzk :
+                          (* ignore this line; it's to work around lack of fixpoint refolding in type inference *) var (type.untranslate _ (type.translate T) * Compilers.type.list (type.untranslate _ (type.translate T)) * type.nat * (type.untranslate _ (type.translate T) -> R))%ctype) ,
+                     (ident.snd @@ Var xyzk)
+                       @ (ident.List_nth_default @@ (ident.fst @@ Var xyzk))
+                | ident.bool_rect T
+                  => λ (xyzk :
+                          (* ignore this line; it's to work around lack of fixpoint refolding in type inference *) var (type.untranslate _ (type.translate T) * type.untranslate _ (type.translate T) * type.bool * (type.untranslate _ (type.translate T) -> R))%ctype) ,
+                     ident.bool_rect
+                       @@ ((ident.snd @@ (Var xyzk))
+                             @ (ident.fst @@ (ident.fst @@ (ident.fst @@ (Var xyzk)))),
+                           (ident.snd @@ (Var xyzk))
+                             @ (ident.snd @@ (ident.fst @@ (ident.fst @@ (Var xyzk)))),
+                           ident.snd @@ (ident.fst @@ (Var xyzk)))
+                | ident.nil t
+                  => λ (_k :
+                          (* ignore this line; it's to work around lack of fixpoint refolding in type inference *) var (() * (Compilers.type.list (type.untranslate _ (type.translate t)) -> R))%ctype) ,
+                     (ident.snd @@ (Var _k))
+                       @ (ident.nil @@ TT)
+                | ident.cons t
+                  => λ (xyk :
+                          (* ignore this line; it's to work around lack of fixpoint refolding in type inference *) var (type.untranslate _ (type.translate t) * Compilers.type.list (type.untranslate _ (type.translate t)) * (Compilers.type.list (type.untranslate _ (type.translate t)) -> R))%ctype) ,
+                     (ident.snd @@ (Var xyk))
+                       @ (ident.cons
+                            @@ (ident.fst @@ (Var xyk)))
+                | ident.fst A B
+                  => λ (xk :
+                          (* ignore this line; it's to work around lack of fixpoint refolding in type inference *) var (type.untranslate _ (type.translate A) * type.untranslate _ (type.translate B) * (type.untranslate _ (type.translate A) -> R))%ctype) ,
+                     (ident.snd @@ (Var xk))
+                       @ (ident.fst
+                            @@ (ident.fst @@ (Var xk)))
+                | ident.snd A B
+                  => λ (xk :
+                          (* ignore this line; it's to work around lack of fixpoint refolding in type inference *) var (type.untranslate _ (type.translate A) * type.untranslate _ (type.translate B) * (type.untranslate _ (type.translate B) -> R))%ctype) ,
+                     (ident.snd @@ (Var xk))
+                       @ (ident.snd
+                            @@ (ident.fst @@ (Var xk)))
+                | ident.Nat_succ as idc
+                | ident.pred as idc
+                  => λ (xyk :
+                          (* ignore this line; it's to work around lack of fixpoint refolding in type inference *) var (type.nat * (type.nat -> R))%ctype) ,
+                     (ident.snd @@ (Var xyk))
+                       @ ((idc : default.ident _ type.nat)
+                            @@ (ident.fst @@ (Var xyk)))
+                | ident.Z_opp as idc
+                  => λ (xyk :
+                          (* ignore this line; it's to work around lack of fixpoint refolding in type inference *) var (type.Z * (type.Z -> R))%ctype) ,
+                     (ident.snd @@ (Var xyk))
+                       @ ((idc : default.ident _ type.Z)
+                            @@ (ident.fst @@ (Var xyk)))
+                | ident.Z_runtime_mul as idc
+                | ident.Z_runtime_add as idc
+                | ident.Z_add as idc
+                | ident.Z_mul as idc
+                | ident.Z_pow as idc
+                | ident.Z_div as idc
+                | ident.Z_modulo as idc
+                  => λ (xyk :
+                          (* ignore this line; it's to work around lack of fixpoint refolding in type inference *) var (type.Z * type.Z * (type.Z -> R))%ctype) ,
+                     (ident.snd @@ (Var xyk))
+                       @ ((idc : default.ident _ type.Z)
+                            @@ (ident.fst @@ (Var xyk)))
+                | ident.Z_eqb as idc
+                  => λ (xyk :
+                          (* ignore this line; it's to work around lack of fixpoint refolding in type inference *) var (type.Z * type.Z * (type.bool -> R))%ctype) ,
+                     (ident.snd @@ (Var xyk))
+                       @ ((idc : default.ident _ type.bool)
+                            @@ (ident.fst @@ (Var xyk)))
+                | ident.Z_of_nat as idc
+                  => λ (xyk :
+                          (* ignore this line; it's to work around lack of fixpoint refolding in type inference *) var (type.nat * (type.Z -> R))%ctype) ,
+                     (ident.snd @@ (Var xyk))
+                       @ ((idc : default.ident _ type.Z)
+                            @@ (ident.fst @@ (Var xyk)))
+                end%expr
+              end.
+    End ident.
+    Notation ident := ident.ident.
+
+    Module default.
+      Notation expr := (@Output.expr.expr ident).
+      Notation Expr := (@Output.expr.Expr ident).
+
+      Definition Translate
+                 {t} (e : @Compilers.Uncurried.expr.default.Expr t)
+        : Expr (type.translate t)
+        := expr.Translate (@ident.wrap) e.
+
+      Definition call_with_continuation
+                 {var}
+                 {R : Compilers.type.type}
+                 {t} (e : @expr _ t)
+                 (k : @Uncurried.expr.default.expr var (type.untranslate R t) -> @Uncurried.expr.default.expr var R)
+        : @Compilers.Uncurried.expr.default.expr var R
+        := expr.call_with_continuation (fun t idc => @ident.untranslate _ t idc _) (@ident.fst) (@ident.snd) e k.
+
+      Definition CallWithContinuation
+                 {R : Compilers.type.type}
+                 {t} (e : Expr t)
+                 (k : forall var, @Uncurried.expr.default.expr var (type.untranslate R t) -> @Uncurried.expr.default.expr var R)
+        : @Compilers.Uncurried.expr.default.Expr R
+        := expr.CallWithContinuation (@ident.untranslate _) (@ident.fst) (@ident.snd) e k.
+
+      Definition CallFunWithIdContinuation'
+                 {R}
+                 {s d} (e : Expr (type.translate (s -> d)))
+                 (k : forall var, var (type.untranslate R (type.translate d)) -> var R)
+        : @Compilers.Uncurried.expr.default.Expr (type.untranslate R (type.translate s) -> R)
+        := fun var
+           => Abs (fun x => @call_with_continuation
+                              var R _ (e _)
+                              (fun e : expr.default.expr (type.untranslate _ (type.translate s) * (type.untranslate _ (type.translate d) -> _) -> _)
+                               => e @ (Var x, λ v , Var (k _ v)))%expr).
+      Notation CallFunWithIdContinuation e
+        := (@CallFunWithIdContinuation'
+              ((fun s d (e' : Expr (type.translate (s -> d))) => d) _ _ e)
+              _ _
+              e
+              (fun _ => id))
+             (only parsing).
+    End default.
+    Include default.
   End CPS.
 
+  Import Uncurried.
   Section invert.
     Context {var : type -> Type}.
 
@@ -1401,6 +1882,11 @@ Module Compilers.
                    end) (only parsing).
     Local Notation if_arrow_s f := (if_arrow (fun s d => f s)) (only parsing).
     Local Notation if_arrow_d f := (if_arrow (fun s d => f d)) (only parsing).
+    Local Notation if_prod f
+      := (fun t => match t return Type with
+                   | type.prod A B => f A B
+                   | _ => True
+                   end).
 
     Definition invert_Abs {s d} (e : @expr var (type.arrow s d)) : option (var s -> @expr var d)
       := match e in expr.expr t return option (if_arrow (fun _ _ => _) t) with
@@ -1414,20 +1900,11 @@ Module Compilers.
          | _ => None
          end.
 
-    Definition invert_Ident {t} (e : @expr var t) : option (ident t)
+    Definition invert_AppIdent {d} (e : @expr var d) : option { s : _ & @ident s d * @expr var s }%type
       := match e with
-         | Ident t idc => Some idc
+         | AppIdent s d idc args
+           => Some (existT _ s (idc, args))
          | _ => None
-         end.
-
-    Definition invert_AppIdent {d} (e : @expr var d) : option { s : _ & @ident (s -> d) * @expr var s }%type
-      := match invert_App e with
-         | Some (existT s (f, x))
-           => match invert_Ident f with
-              | Some f' => Some (existT _ s (f', x))
-              | None => None
-              end
-         | None => None
          end.
 
     Definition invert_App2 {d} (e : @expr var d) : option { s1s2 : _ * _ & @expr var (fst s1s2 -> snd s1s2 -> d) * @expr var (fst s1s2) * @expr var (snd s1s2) }%type
@@ -1448,30 +1925,19 @@ Module Compilers.
                    end) (only parsing).
 
     Definition invert_Pair {A B} (e : @expr var (type.prod A B)) : option (@expr var A * @expr var B)
-      := match invert_App2 e with
-         | Some (existT (s1, s2) (f, x, y))
-           => match invert_Ident f with
-              | Some idc
-                => match idc in ident t
-                         return if_arrow_s expr t
-                                -> if_arrow_d (if_arrow_s expr) t
-                                -> option (if_arrow_d (if_arrow_d expr_prod) t)
-                   with
-                   | ident.pair A B => fun x y => Some (x, y)
-                   | _ => fun _ _ => None
-                   end x y
-              | None => None
-              end
-         | None => None
+      := match e in expr.expr t return option (if_prod (fun A B => expr A * expr B)%type t) with
+         | Pair A B a b
+           => Some (a, b)
+         | _ => None
          end.
 
     (* if we want more code for the below, I would suggest [reify_base_type] and [reflect_base_type] *)
     Definition reify_primitive {t} (v : type.interp (type.type_primitive t)) : @expr var (type.type_primitive t)
-      := Ident (ident.primitive v).
+      := AppIdent (ident.primitive v) TT.
     Definition reflect_primitive {t} (e : @expr var (type.type_primitive t)) : option (type.interp (type.type_primitive t))
-      := match invert_Ident e with
-         | Some idc
-           => match idc in ident t return option (type.interp t) with
+      := match invert_AppIdent e with
+         | Some (existT s (idc, args))
+           => match idc in ident _ t return option (type.interp t) with
               | ident.primitive _ v => Some v
               | _ => None
               end
@@ -1488,29 +1954,30 @@ Module Compilers.
     Fixpoint reflect_list {t} (e : @expr var (type.list t))
       : option (list (@expr var t))
       := match e in expr.expr t return option (list_expr t) with
-         | Ident t idc
-           => match idc in ident t return option (list_expr t) with
-              | ident.nil _ => Some nil
-              | _ => None
-              end
-         | App (type.list s) d f xs
-               (* WHY reflect xs before x? *)
-           => match @reflect_list s xs return _ with
-              | Some xs
-                => match invert_AppIdent f return option (list_expr d) with
-                   | Some (existT s' (idc, x))
-                     => match idc in ident t
-                              return if_arrow_s expr t
-                                     -> if_arrow_d (if_arrow_s list_expr) t
-                                     -> option (if_arrow_d (if_arrow_d list_expr) t)
-                        with
-                        | ident.cons A => fun x xs => Some (cons x xs)
-                        | _ => fun _ _ => None
-                        end x xs
-                   | _ => None
+         | AppIdent s (type.list t) idc x_xs
+           => match x_xs in expr.expr s return ident s (type.list t) -> option (list (expr t)) with
+              | Pair A (type.list B) x xs
+                => match @reflect_list B xs with
+                   | Some xs
+                     => fun idc
+                        => match idc in ident s d
+                                 return if_prod (fun A B => expr A) s
+                                        -> if_prod (fun A B => list_expr B) s
+                                        -> option (list_expr d)
+                           with
+                           | ident.cons A
+                             => fun x xs => Some (cons x xs)
+                           | _ => fun _ _ => None
+                           end x xs
+                   | None => fun _ => None
                    end
-              | None => None
-              end
+              | _
+                => fun idc
+                   => match idc in ident _ t return option (list_expr t) with
+                      | ident.nil _ => Some nil
+                      | _ => None
+                      end
+              end idc
          | _ => None
          end.
   End invert.
@@ -1520,8 +1987,8 @@ Module Compilers.
     Definition reify_list {t} (ls : list (@expr var t)) : @expr var (type.list t)
       := list_rect
            (fun _ => _)
-           (Ident ident.nil)
-           (fun x _ xs => App (App (Ident ident.cons) x) xs)
+           (ident.nil @@ TT)%expr
+           (fun x _ xs => ident.cons @@ (x, xs))%expr
            ls.
   End gallina_reify.
 
@@ -1575,8 +2042,8 @@ Module Compilers.
                => fun x : expr t + type.interp t
                   => match x with
                      | inl v => v
-                     | inr v => Ident (ident.primitive v)
-                     end
+                     | inr v => ident.primitive v @@ TT
+                     end%expr
              end
         with reflect {t : type}
              : @expr var t -> value var t
@@ -1636,71 +2103,71 @@ Module Compilers.
                      | inr v => f (inr v) (* FIXME: do not substitute [S (big stuck term)] *)
                      end
              end.
-        Definition interp {t} (idc : ident t) : value var t
-          := match idc in ident t return value var t with
-             | ident.Let_In tx tC
-               => interp_let_in
-             | ident.nil t
-               => inr (@nil (value var t))
-             | ident.primitive t v
-               => inr v
-             | ident.cons t as idc
-               => fun x (xs : expr (type.list t) + list (value var t))
-                  => match xs return expr (type.list t) + list (value var t) with
-                     | inr xs => inr (cons x xs)
-                     | _ => expr.reflect (Ident idc) x xs
+        Definition interp {s d} (idc : ident s d) : value var (s -> d)
+          := match idc in ident s d return value var (s -> d) with
+             | ident.Let_In tx tC as idc
+               => fun (xf : expr (tx * (tx -> tC)) + value var tx * value var (tx -> tC))
+                  => match xf with
+                     | inr (x, f) => interp_let_in x f
+                     | _ => expr.reflect (AppIdent idc (expr.reify (t:=tx * (tx -> tC)) xf))
                      end
-             | ident.pair A B as idc
-               => fun x y => @inr _ (value var A * value var B) (x, y)
+             | ident.nil t
+               => fun _ => inr (@nil (value var t))
+             | ident.primitive t v
+               => fun _ => inr v
+             | ident.cons t as idc
+               => fun (x_xs : expr (t * type.list t) + value var t * (expr (type.list t) + list (value var t)))
+                  => match x_xs return expr (type.list t) + list (value var t) with
+                     | inr (x, inr xs) => inr (cons x xs)
+                     | _ => expr.reflect (AppIdent idc (expr.reify (t:=t * type.list t) x_xs))
+                     end
              | ident.fst A B as idc
                => fun x : expr (A * B) + value var A * value var B
                   => match x with
                      | inr x => fst x
-                     | _ => expr.reflect (Ident idc) x
+                     | _ => expr.reflect (AppIdent idc (expr.reify (t:=A*B) x))
                      end
              | ident.snd A B as idc
                => fun x : expr (A * B) + value var A * value var B
                   => match x with
                      | inr x => snd x
-                     | _ => expr.reflect (Ident idc) x
+                     | _ => expr.reflect (AppIdent idc (expr.reify (t:=A*B) x))
                      end
              | ident.bool_rect T as idc
-               => fun true_case false_case (b : expr type.bool + bool)
-                  => match b with
-                     | inr b => @bool_rect (fun _ => value var T) true_case false_case b
-                     | _ => expr.reflect (Ident idc) true_case false_case b
+               => fun (true_case_false_case_b : expr (T * T * type.bool) + (expr (T * T) + value var T * value var T) * (expr type.bool + bool))
+                  => match true_case_false_case_b with
+                     | inr (inr (true_case, false_case), inr b)
+                       => @bool_rect (fun _ => value var T) true_case false_case b
+                     | _ => expr.reflect (AppIdent idc (expr.reify (t:=T*T*type.bool) true_case_false_case_b))
                      end
              | ident.nat_rect P as idc
-               => fun (O_case : value var P)
-                      (S_case : expr type.nat + nat -> value var P -> value var P)
-                      (n : expr type.nat + nat)
-                  => match n with
-                     | inr n => @nat_rect (fun _ => value var P)
-                                          O_case
-                                          (fun n' => S_case (inr n'))
-                                          n
-                     | _ => expr.reflect (Ident idc) O_case S_case n
+               => fun (O_case_S_case_n : expr (P * (type.nat * P -> P) * type.nat) + (expr (P * (type.nat * P -> P)) + value var P * value var (type.nat * P -> P)) * (expr type.nat + nat))
+                  => match O_case_S_case_n with
+                     | inr (inr (O_case, S_case), inr n)
+                       => @nat_rect (fun _ => value var P)
+                                    O_case
+                                    (fun n' rec => S_case (inr (inr n', rec)))
+                                    n
+                     | _ => expr.reflect (AppIdent idc (expr.reify (t:=P * (type.nat * P -> P) * type.nat) O_case_S_case_n))
                      end
              | ident.list_rect A P as idc
-               => fun (nil_case : value var P)
-                      (cons_case : value var A -> expr (type.list A) + list (value var A) -> value var P -> value var P)
-                      (ls : expr (type.list A) + list (value var A))
-                  => match ls with
-                     | inr ls => @list_rect
-                                   (value var A)
-                                   (fun _ => value var P)
-                                   nil_case
-                                   (fun x xs rec => cons_case x (inr xs) rec)
-                                   ls
-                     | _ => expr.reflect (Ident idc) nil_case cons_case ls
+               => fun (nil_case_cons_case_ls : expr (P * (A * type.list A * P -> P) * type.list A) + (expr (P * (A * type.list A * P -> P)) + value var P * value var (A * type.list A * P -> P)) * (expr (type.list A) + list (value var A)))
+                  => match nil_case_cons_case_ls with
+                     | inr (inr (nil_case, cons_case), inr ls)
+                       => @list_rect
+                            (value var A)
+                            (fun _ => value var P)
+                            nil_case
+                            (fun x xs rec => cons_case (inr (inr (x, inr xs), rec)))
+                            ls
+                     | _ => expr.reflect (AppIdent idc (expr.reify (t:=P * (A * type.list A * P -> P) * type.list A) nil_case_cons_case_ls))
                      end
              | ident.List.nth_default A as idc
-               => fun (default : value var A)
-                      (ls : expr _ + list (value var A))
-                      (idx : expr _ + nat)
-                  => match ls, idx return value var A with
-                     | inr ls, inr idx => List.nth_default default ls idx
-                     | _, _ => expr.reflect (Ident idc) default ls idx
+               => fun (default_ls_idx : expr (A * type.list A * type.nat) + (expr (A * type.list A) + value var A * (expr (type.list A) + list (value var A))) * (expr type.nat + nat))
+                  => match default_ls_idx with
+                     | inr (inr (default, inr ls), inr idx)
+                       => List.nth_default default ls idx
+                     | _ => expr.reflect (AppIdent idc (expr.reify (t:=A * type.list A * type.nat) default_ls_idx))
                      end
              | ident.pred as idc
              | ident.Nat_succ as idc
@@ -1709,7 +2176,7 @@ Module Compilers.
                => fun x : expr _ + type.interp _
                   => match x return expr _ + type.interp _ with
                      | inr x => inr (ident.interp idc x)
-                     | _ => expr.reflect (Ident idc) x
+                     | inl x => expr.reflect (AppIdent idc x)
                      end
              | ident.Z_add as idc
              | ident.Z_mul as idc
@@ -1717,38 +2184,38 @@ Module Compilers.
              | ident.Z_div as idc
              | ident.Z_modulo as idc
              | ident.Z_eqb as idc
-               => fun (x y : expr _ + type.interp _)
-                  => match x, y return expr _ + type.interp _ with
-                     | inr x, inr y => inr (ident.interp idc x y)
-                     | _, _ => expr.reflect (Ident idc) x y
+               => fun (x_y : expr (_ * _) + (expr _ + type.interp _) * (expr _ + type.interp _))
+                  => match x_y return expr _ + type.interp _ with
+                     | inr (inr x, inr y) => inr (ident.interp idc (x, y))
+                     | _ => expr.reflect (AppIdent idc (expr.reify (t:=_*_) x_y))
                      end
              | ident.Z_runtime_mul as idc
-               => fun (x y : expr _ + type.interp _)
-                  => let default := expr.reflect (Ident idc) x y in
-                     match x, y return expr _ + type.interp _ with
-                     | inr x, inr y => inr (ident.interp idc x y)
-                     | inr x, inl e
-                     | inl e, inr x
+               => fun (x_y : expr (_ * _) + (expr _ + type.interp _) * (expr _ + type.interp _))
+                  => let default := expr.reflect (AppIdent idc (expr.reify (t:=_*_) x_y)) in
+                     match x_y return expr _ + type.interp _ with
+                     | inr (inr x, inr y) => inr (ident.interp idc (x, y))
+                     | inr (inr x, inl e)
+                     | inr (inl e, inr x)
                        => if Z.eqb x 0
                           then inr 0%Z
                           else if Z.eqb x 1
                                then inl e
                                else default
-                     | inl _, inl _ => default
+                     | inr (inl _, inl _) | inl _ => default
                      end
              | ident.Z_runtime_add as idc
-               => fun (x y : expr _ + type.interp _)
-                  => let default := expr.reflect (Ident idc) x y in
-                     match x, y return expr _ + type.interp _ with
-                     | inr x, inr y => inr (ident.interp idc x y)
-                     | inr x, inl e
-                     | inl e, inr x
+               => fun (x_y : expr (_ * _) + (expr _ + type.interp _) * (expr _ + type.interp _))
+                  => let default := expr.reflect (AppIdent idc (expr.reify (t:=_*_) x_y)) in
+                     match x_y return expr _ + type.interp _ with
+                     | inr (inr x, inr y) => inr (ident.interp idc (x, y))
+                     | inr (inr x, inl e)
+                     | inr (inl e, inr x)
                        => if Z.eqb x 0
                           then inl e
                           else default
-                     | inl _, inl _ => default
+                     | inr (inl _, inl _) | inl _ => default
                      end
-                 end.
+             end.
       End interp.
     End ident.
   End partial.
@@ -1760,7 +2227,9 @@ Module Compilers.
       : partial.value var t
       := match e in expr.expr t return partial.value var t with
          | Var t v => v
-         | Ident t idc => partial.ident.interp idc
+         | TT => inr tt
+         | AppIdent s d idc args => partial.ident.interp idc (@partial_reduce' _ args)
+         | Pair A B a b => inr (@partial_reduce' A a, @partial_reduce' B b)
          | App s d f x => @partial_reduce' _ f (@partial_reduce' _ x)
          | Abs s d f => fun x => @partial_reduce' d (f x)
          end.
@@ -1810,20 +2279,21 @@ Proof.
 Qed.
 
 Delimit Scope RT_expr_scope with RT_expr.
+Import Uncurried.
 Import expr.
 Import for_reification.Notations.Reification.
 
 Notation "x + y"
-  := (App (App (Ident ident.Z.runtime_add) x%RT_expr) y%RT_expr)
+  := (AppIdent ident.Z.runtime_add (x%RT_expr, y%RT_expr)%expr)
      : RT_expr_scope.
 Notation "x * y"
-  := (App (App (Ident ident.Z.runtime_mul) x%RT_expr) y%RT_expr)
+  := (AppIdent ident.Z.runtime_mul (x%RT_expr, y%RT_expr)%expr)
      : RT_expr_scope.
 Notation "x + y"
-  := (App (App (Ident ident.Z.runtime_add) x%RT_expr) y%RT_expr)
+  := (AppIdent ident.Z.runtime_add (x%RT_expr, y%RT_expr)%expr)
      : expr_scope.
 Notation "x * y"
-  := (App (App (Ident ident.Z.runtime_mul) x%RT_expr) y%RT_expr)
+  := (AppIdent ident.Z.runtime_mul (x%RT_expr, y%RT_expr)%expr)
      : expr_scope.
 Notation "x" := (Var x) (only printing, at level 9) : expr_scope.
 Open Scope RT_expr_scope.
@@ -1834,7 +2304,8 @@ Require Import AdmitAxiom.
 Definition w (i:nat) : Z := 2^Qceiling(51*i).
 Example base_51_carry_mul (*(f0 f1 f2 f3 f4 f5 f6 f7 f8 f9 g0 g1 g2 g3 g4 g5 g6 g7 g8 g9 : Z)
         (f:=(f0 :: f1 :: f2 :: f3 :: f4 :: f5 :: f6 :: f7 :: f8 :: f9 :: nil)%list)
-        (g:=(f0 :: f1 :: f2 :: f3 :: f4 :: f5 :: f6 :: f7 :: f8 :: f9 :: nil)%list)*) (f g : list Z)
+        (g:=(f0 :: f1 :: f2 :: f3 :: f4 :: f5 :: f6 :: f7 :: f8 :: f9 :: nil)%list)*) (fg : list Z * list Z)
+        (f := fst fg) (g := snd fg)
         (n:=5%nat)
         (Hf : length f = n) (Hg : length g = n)
   : { fg : list Z | (eval w n fg) mod (2^255-19)
@@ -1849,7 +2320,7 @@ Example base_51_carry_mul (*(f0 f1 f2 f3 f4 f5 f6 f7 f8 f9 g0 g1 g2 g3 g4 g5 g6 
 (*        (g9,g8,g7,g6,g5,g4,g3,g2,g1,g0)) mod (2^255 - 19) *)
   etransitivity; (* work around [rewrite] being stupid about evars *)
     [
-    | rewrite <- eval_chained_carries with (s:=2^255) (c:=[(1,19)]) (idxs:=(seq 0 (pred n) ++ [0; 1])%list%nat) (modulo:=Z.modulo) (div:=Z.div)
+    | rewrite <- eval_chained_carries with (s:=2^255) (c:=[(1,19)]) (idxs:=(seq 0 (pred n) ++ [0; 1])%list%nat) (modulo:=fun x y => Z.modulo x y) (div:=fun x y => Z.div x y)
       by (try assumption; auto using Z.div_mod; try (intros; eapply pow_ceil_mul_nat_divide_nonzero); try eapply pow_ceil_mul_nat_nonzero; try vm_decide);
       reflexivity ].
   eapply f_equal2; [|trivial]. eapply f_equal.
@@ -1863,11 +2334,11 @@ Example base_51_carry_mul (*(f0 f1 f2 f3 f4 f5 f6 f7 f8 f9 g0 g1 g2 g3 g4 g5 g6 
   rewrite <- (expand_list_correct n (-1)%Z f), <- (expand_list_correct n (-1)%Z g) by assumption; subst e.
   etransitivity.
   Focus 2.
-  {
-    repeat match goal with H : _ |- _ => clear H end; revert f g.
+  { subst f g.
+    repeat match goal with H : _ |- _ => clear H end; revert fg.
     lazymatch goal with
-    | [ |- forall f g, ?ev = @?RHS f g ]
-      => refine (fun f g => f_equal (fun F => F f g) (_ : _ = RHS))
+    | [ |- forall fg, ?ev = @?RHS fg ]
+      => refine (fun fg => f_equal (fun F => F fg) (_ : _ = RHS))
     end.
     cbv [n expand_list expand_list_helper].
     cbv delta [chained_carries carry carry_reduce Associational.carry carryterm mulmod w to_associational mul to_associational reduce from_associational add_to_nth zeros place split].
@@ -1879,7 +2350,7 @@ Example base_51_carry_mul (*(f0 f1 f2 f3 f4 f5 f6 f7 f8 f9 g0 g1 g2 g3 g4 g5 g6 
       pose (PartialReduce (canonicalize_list_recursion E)) as E'.
       vm_compute in E'.
       lazymatch (eval cbv delta [E'] in E') with
-      | (fun var => Ident (ident.primitive ?v)) => idtac
+      | (fun var => AppIdent (ident.primitive ?v) TT) => idtac
       end.
       constructor. }
     assert True.
@@ -1910,9 +2381,11 @@ Example base_51_carry_mul (*(f0 f1 f2 f3 f4 f5 f6 f7 f8 f9 g0 g1 g2 g3 g4 g5 g6 
                          (z * z)%RT) in
       pose v as E.
       vm_compute in E.
-      pose (PartialReduce (CPS.expr.TranslateUnderBinders (canonicalize_list_recursion E) (fun var => (tt, id, id)))) as E'.
+      pose (CPS.CallFunWithIdContinuation (CPS.Translate (canonicalize_list_recursion E))) as E'.
       vm_compute in E'.
-      lazymatch (eval cbv delta [E'] in E') with
+      pose (PartialReduce E') as E''.
+      lazy in E''.
+      lazymatch (eval cbv delta [E''] in E'') with
       | (fun var : type -> Type =>
            (λ x : var (type.type_primitive type.Z),
                   expr_let x0 := Var x * Var x in
@@ -1927,12 +2400,12 @@ Example base_51_carry_mul (*(f0 f1 f2 f3 f4 f5 f6 f7 f8 f9 g0 g1 g2 g3 g4 g5 g6 
     reflexivity.
   } Unfocus.
   cbv beta.
-  let e := match goal with |- _ = expr.Interp _ ?e _ _ => e end in
+  let e := match goal with |- _ = expr.Interp _ ?e _ => e end in
   set (E := e).
-  Time let E' := constr:(PartialReduce (CPS.expr.TranslateUnderBinders (canonicalize_list_recursion E) (fun var => (tt, id, id, id)))) in
+  Time let E' := constr:(PartialReduce (CPS.CallFunWithIdContinuation (CPS.Translate (canonicalize_list_recursion E)))) in
        let E' := (eval lazy in E') in
        pose E' as E''.
-  transitivity (Interp E'' f g); [ clear E | admit ].
+  transitivity (Interp E'' fg); [ clear E | admit ].
   reflexivity.
   (*cbv -[runtime_mul runtime_add]; cbv [runtime_mul runtime_add].
   ring_simplify_subterms.*)
@@ -1949,154 +2422,169 @@ Example base_51_carry_mul (*(f0 f1 f2 f3 f4 f5 f6 f7 f8 f9 g0 g1 g2 g3 g4 g5 g6 
   f0*g0+ 38*f1*g9+ 19*f2*g8+ 38*f3*g7+ 19*f4*g6+ 38*f5*g5+ 19*f6*g4+ 38*f7*g3+ 19*f8*g2+ 38*f9*g1) *)
   (*trivial.*)
 Defined.
-Eval cbv [proj1_sig base_51_carry_mul] in (fun f g Hf Hg => proj1_sig (base_51_carry_mul f g Hf Hg)).
-(*     = fun (f g : list Z) (_ : length f = 5%nat) (_ : length g = 5%nat) =>
-       expr.Interp (@ident.interp)
+Import ident.
+Eval cbv [proj1_sig base_51_carry_mul] in (fun fg Hf Hg => proj1_sig (base_51_carry_mul fg Hf Hg)).
+(*     = fun (fg : list Z * list Z) (_ : length (Datatypes.fst fg) = 5%nat)
+         (_ : length (Datatypes.snd fg) = 5%nat) =>
+       expr.Interp (@interp)
          (fun var : type -> Type =>
-          (λ x x0 : var (type.list type.Z),
-           expr_let y := x [[0]] * x0 [[4]] +
-                         (x [[1]] * x0 [[3]] +
-                          (x [[2]] * x0 [[2]] +
-                           (x [[3]] * x0 [[1]] + x [[4]] * x0 [[0]]))) in
-           expr_let _ := Ident ident.Z.div @ y @ 2251799813685248 in
-           expr_let _ := Ident ident.Z.modulo @ y @ 2251799813685248 in
-           expr_let y2 := x [[0]] * x0 [[3]] +
-                          (x [[1]] * x0 [[2]] +
-                           (x [[2]] * x0 [[1]] +
-                            (x [[3]] * x0 [[0]] + 19 * (x [[4]] * x0 [[4]])))) in
-           expr_let _ := Ident ident.Z.div @ y2 @ 2251799813685248 in
-           expr_let _ := Ident ident.Z.modulo @ y2 @ 2251799813685248 in
-           expr_let y5 := x [[0]] * x0 [[2]] +
-                          (x [[1]] * x0 [[1]] +
-                           (x [[2]] * x0 [[0]] +
-                            (19 * (x [[3]] * x0 [[4]]) + 19 * (x [[4]] * x0 [[3]])))) in
-           expr_let _ := Ident ident.Z.div @ y5 @ 2251799813685248 in
-           expr_let _ := Ident ident.Z.modulo @ y5 @ 2251799813685248 in
-           expr_let y8 := x [[0]] * x0 [[1]] +
-                          (x [[1]] * x0 [[0]] +
-                           (19 * (x [[2]] * x0 [[4]]) +
-                            (19 * (x [[3]] * x0 [[3]]) + 19 * (x [[4]] * x0 [[2]])))) in
-           expr_let _ := Ident ident.Z.div @ y8 @ 2251799813685248 in
-           expr_let _ := Ident ident.Z.modulo @ y8 @ 2251799813685248 in
-           expr_let y11 := x [[0]] * x0 [[0]] +
-                           (19 * (x [[1]] * x0 [[4]]) +
-                            (19 * (x [[2]] * x0 [[3]]) +
-                             (19 * (x [[3]] * x0 [[2]]) +
-                              19 * (x [[4]] * x0 [[1]])))) in
-           expr_let y12 := Ident ident.Z.div @ y11 @ 2251799813685248 in
-           expr_let y13 := Ident ident.Z.modulo @ y11 @ 2251799813685248 in
-           expr_let y14 := x [[0]] * x0 [[4]] +
-                           (x [[1]] * x0 [[3]] +
-                            (x [[2]] * x0 [[2]] +
-                             (x [[3]] * x0 [[1]] + x [[4]] * x0 [[0]]))) in
-           expr_let _ := Ident ident.Z.div @ y14 @ 2251799813685248 in
-           expr_let _ := Ident ident.Z.modulo @ y14 @ 2251799813685248 in
-           expr_let y17 := x [[0]] * x0 [[3]] +
-                           (x [[1]] * x0 [[2]] +
-                            (x [[2]] * x0 [[1]] +
-                             (x [[3]] * x0 [[0]] + 19 * (x [[4]] * x0 [[4]])))) in
-           expr_let _ := Ident ident.Z.div @ y17 @ 2251799813685248 in
-           expr_let _ := Ident ident.Z.modulo @ y17 @ 2251799813685248 in
-           expr_let y20 := x [[0]] * x0 [[2]] +
-                           (x [[1]] * x0 [[1]] +
-                            (x [[2]] * x0 [[0]] +
-                             (19 * (x [[3]] * x0 [[4]]) +
-                              19 * (x [[4]] * x0 [[3]])))) in
-           expr_let _ := Ident ident.Z.div @ y20 @ 2251799813685248 in
-           expr_let _ := Ident ident.Z.modulo @ y20 @ 2251799813685248 in
+          (λ x : var (type.list type.Z * type.list type.Z)%ctype,
+           expr_let y := fst @@ x [[0]] * snd @@ x [[4]] +
+                         (fst @@ x [[1]] * snd @@ x [[3]] +
+                          (fst @@ x [[2]] * snd @@ x [[2]] +
+                           (fst @@ x [[3]] * snd @@ x [[1]] +
+                            fst @@ x [[4]] * snd @@ x [[0]]))) in
+           expr_let _ := Z.div @@ (y, 2251799813685248) in
+           expr_let _ := Z.modulo @@ (y, 2251799813685248) in
+           expr_let y2 := fst @@ x [[0]] * snd @@ x [[3]] +
+                          (fst @@ x [[1]] * snd @@ x [[2]] +
+                           (fst @@ x [[2]] * snd @@ x [[1]] +
+                            (fst @@ x [[3]] * snd @@ x [[0]] +
+                             19 * (fst @@ x [[4]] * snd @@ x [[4]])))) in
+           expr_let _ := Z.div @@ (y2, 2251799813685248) in
+           expr_let _ := Z.modulo @@ (y2, 2251799813685248) in
+           expr_let y5 := fst @@ x [[0]] * snd @@ x [[2]] +
+                          (fst @@ x [[1]] * snd @@ x [[1]] +
+                           (fst @@ x [[2]] * snd @@ x [[0]] +
+                            (19 * (fst @@ x [[3]] * snd @@ x [[4]]) +
+                             19 * (fst @@ x [[4]] * snd @@ x [[3]])))) in
+           expr_let _ := Z.div @@ (y5, 2251799813685248) in
+           expr_let _ := Z.modulo @@ (y5, 2251799813685248) in
+           expr_let y8 := fst @@ x [[0]] * snd @@ x [[1]] +
+                          (fst @@ x [[1]] * snd @@ x [[0]] +
+                           (19 * (fst @@ x [[2]] * snd @@ x [[4]]) +
+                            (19 * (fst @@ x [[3]] * snd @@ x [[3]]) +
+                             19 * (fst @@ x [[4]] * snd @@ x [[2]])))) in
+           expr_let _ := Z.div @@ (y8, 2251799813685248) in
+           expr_let _ := Z.modulo @@ (y8, 2251799813685248) in
+           expr_let y11 := fst @@ x [[0]] * snd @@ x [[0]] +
+                           (19 * (fst @@ x [[1]] * snd @@ x [[4]]) +
+                            (19 * (fst @@ x [[2]] * snd @@ x [[3]]) +
+                             (19 * (fst @@ x [[3]] * snd @@ x [[2]]) +
+                              19 * (fst @@ x [[4]] * snd @@ x [[1]])))) in
+           expr_let y12 := Z.div @@ (y11, 2251799813685248) in
+           expr_let y13 := Z.modulo @@ (y11, 2251799813685248) in
+           expr_let y14 := fst @@ x [[0]] * snd @@ x [[4]] +
+                           (fst @@ x [[1]] * snd @@ x [[3]] +
+                            (fst @@ x [[2]] * snd @@ x [[2]] +
+                             (fst @@ x [[3]] * snd @@ x [[1]] +
+                              fst @@ x [[4]] * snd @@ x [[0]]))) in
+           expr_let _ := Z.div @@ (y14, 2251799813685248) in
+           expr_let _ := Z.modulo @@ (y14, 2251799813685248) in
+           expr_let y17 := fst @@ x [[0]] * snd @@ x [[3]] +
+                           (fst @@ x [[1]] * snd @@ x [[2]] +
+                            (fst @@ x [[2]] * snd @@ x [[1]] +
+                             (fst @@ x [[3]] * snd @@ x [[0]] +
+                              19 * (fst @@ x [[4]] * snd @@ x [[4]])))) in
+           expr_let _ := Z.div @@ (y17, 2251799813685248) in
+           expr_let _ := Z.modulo @@ (y17, 2251799813685248) in
+           expr_let y20 := fst @@ x [[0]] * snd @@ x [[2]] +
+                           (fst @@ x [[1]] * snd @@ x [[1]] +
+                            (fst @@ x [[2]] * snd @@ x [[0]] +
+                             (19 * (fst @@ x [[3]] * snd @@ x [[4]]) +
+                              19 * (fst @@ x [[4]] * snd @@ x [[3]])))) in
+           expr_let _ := Z.div @@ (y20, 2251799813685248) in
+           expr_let _ := Z.modulo @@ (y20, 2251799813685248) in
            expr_let y23 := y12 +
-                           (x [[0]] * x0 [[1]] +
-                            (x [[1]] * x0 [[0]] +
-                             (19 * (x [[2]] * x0 [[4]]) +
-                              (19 * (x [[3]] * x0 [[3]]) +
-                               19 * (x [[4]] * x0 [[2]]))))) in
-           expr_let y24 := Ident ident.Z.div @ y23 @ 2251799813685248 in
-           expr_let y25 := Ident ident.Z.modulo @ y23 @ 2251799813685248 in
-           expr_let _ := Ident ident.Z.div @ y13 @ 2251799813685248 in
-           expr_let _ := Ident ident.Z.modulo @ y13 @ 2251799813685248 in
-           expr_let y28 := x [[0]] * x0 [[4]] +
-                           (x [[1]] * x0 [[3]] +
-                            (x [[2]] * x0 [[2]] +
-                             (x [[3]] * x0 [[1]] + x [[4]] * x0 [[0]]))) in
-           expr_let _ := Ident ident.Z.div @ y28 @ 2251799813685248 in
-           expr_let _ := Ident ident.Z.modulo @ y28 @ 2251799813685248 in
-           expr_let y31 := x [[0]] * x0 [[3]] +
-                           (x [[1]] * x0 [[2]] +
-                            (x [[2]] * x0 [[1]] +
-                             (x [[3]] * x0 [[0]] + 19 * (x [[4]] * x0 [[4]])))) in
-           expr_let _ := Ident ident.Z.div @ y31 @ 2251799813685248 in
-           expr_let _ := Ident ident.Z.modulo @ y31 @ 2251799813685248 in
+                           (fst @@ x [[0]] * snd @@ x [[1]] +
+                            (fst @@ x [[1]] * snd @@ x [[0]] +
+                             (19 * (fst @@ x [[2]] * snd @@ x [[4]]) +
+                              (19 * (fst @@ x [[3]] * snd @@ x [[3]]) +
+                               19 * (fst @@ x [[4]] * snd @@ x [[2]]))))) in
+           expr_let y24 := Z.div @@ (y23, 2251799813685248) in
+           expr_let y25 := Z.modulo @@ (y23, 2251799813685248) in
+           expr_let _ := Z.div @@ (y13, 2251799813685248) in
+           expr_let _ := Z.modulo @@ (y13, 2251799813685248) in
+           expr_let y28 := fst @@ x [[0]] * snd @@ x [[4]] +
+                           (fst @@ x [[1]] * snd @@ x [[3]] +
+                            (fst @@ x [[2]] * snd @@ x [[2]] +
+                             (fst @@ x [[3]] * snd @@ x [[1]] +
+                              fst @@ x [[4]] * snd @@ x [[0]]))) in
+           expr_let _ := Z.div @@ (y28, 2251799813685248) in
+           expr_let _ := Z.modulo @@ (y28, 2251799813685248) in
+           expr_let y31 := fst @@ x [[0]] * snd @@ x [[3]] +
+                           (fst @@ x [[1]] * snd @@ x [[2]] +
+                            (fst @@ x [[2]] * snd @@ x [[1]] +
+                             (fst @@ x [[3]] * snd @@ x [[0]] +
+                              19 * (fst @@ x [[4]] * snd @@ x [[4]])))) in
+           expr_let _ := Z.div @@ (y31, 2251799813685248) in
+           expr_let _ := Z.modulo @@ (y31, 2251799813685248) in
            expr_let y34 := y24 +
-                           (x [[0]] * x0 [[2]] +
-                            (x [[1]] * x0 [[1]] +
-                             (x [[2]] * x0 [[0]] +
-                              (19 * (x [[3]] * x0 [[4]]) +
-                               19 * (x [[4]] * x0 [[3]]))))) in
-           expr_let y35 := Ident ident.Z.div @ y34 @ 2251799813685248 in
-           expr_let y36 := Ident ident.Z.modulo @ y34 @ 2251799813685248 in
-           expr_let _ := Ident ident.Z.div @ y25 @ 2251799813685248 in
-           expr_let _ := Ident ident.Z.modulo @ y25 @ 2251799813685248 in
-           expr_let _ := Ident ident.Z.div @ y13 @ 2251799813685248 in
-           expr_let _ := Ident ident.Z.modulo @ y13 @ 2251799813685248 in
-           expr_let y41 := x [[0]] * x0 [[4]] +
-                           (x [[1]] * x0 [[3]] +
-                            (x [[2]] * x0 [[2]] +
-                             (x [[3]] * x0 [[1]] + x [[4]] * x0 [[0]]))) in
-           expr_let _ := Ident ident.Z.div @ y41 @ 2251799813685248 in
-           expr_let _ := Ident ident.Z.modulo @ y41 @ 2251799813685248 in
+                           (fst @@ x [[0]] * snd @@ x [[2]] +
+                            (fst @@ x [[1]] * snd @@ x [[1]] +
+                             (fst @@ x [[2]] * snd @@ x [[0]] +
+                              (19 * (fst @@ x [[3]] * snd @@ x [[4]]) +
+                               19 * (fst @@ x [[4]] * snd @@ x [[3]]))))) in
+           expr_let y35 := Z.div @@ (y34, 2251799813685248) in
+           expr_let y36 := Z.modulo @@ (y34, 2251799813685248) in
+           expr_let _ := Z.div @@ (y25, 2251799813685248) in
+           expr_let _ := Z.modulo @@ (y25, 2251799813685248) in
+           expr_let _ := Z.div @@ (y13, 2251799813685248) in
+           expr_let _ := Z.modulo @@ (y13, 2251799813685248) in
+           expr_let y41 := fst @@ x [[0]] * snd @@ x [[4]] +
+                           (fst @@ x [[1]] * snd @@ x [[3]] +
+                            (fst @@ x [[2]] * snd @@ x [[2]] +
+                             (fst @@ x [[3]] * snd @@ x [[1]] +
+                              fst @@ x [[4]] * snd @@ x [[0]]))) in
+           expr_let _ := Z.div @@ (y41, 2251799813685248) in
+           expr_let _ := Z.modulo @@ (y41, 2251799813685248) in
            expr_let y44 := y35 +
-                           (x [[0]] * x0 [[3]] +
-                            (x [[1]] * x0 [[2]] +
-                             (x [[2]] * x0 [[1]] +
-                              (x [[3]] * x0 [[0]] + 19 * (x [[4]] * x0 [[4]]))))) in
-           expr_let y45 := Ident ident.Z.div @ y44 @ 2251799813685248 in
-           expr_let y46 := Ident ident.Z.modulo @ y44 @ 2251799813685248 in
-           expr_let _ := Ident ident.Z.div @ y36 @ 2251799813685248 in
-           expr_let _ := Ident ident.Z.modulo @ y36 @ 2251799813685248 in
-           expr_let _ := Ident ident.Z.div @ y25 @ 2251799813685248 in
-           expr_let _ := Ident ident.Z.modulo @ y25 @ 2251799813685248 in
-           expr_let _ := Ident ident.Z.div @ y13 @ 2251799813685248 in
-           expr_let _ := Ident ident.Z.modulo @ y13 @ 2251799813685248 in
+                           (fst @@ x [[0]] * snd @@ x [[3]] +
+                            (fst @@ x [[1]] * snd @@ x [[2]] +
+                             (fst @@ x [[2]] * snd @@ x [[1]] +
+                              (fst @@ x [[3]] * snd @@ x [[0]] +
+                               19 * (fst @@ x [[4]] * snd @@ x [[4]]))))) in
+           expr_let y45 := Z.div @@ (y44, 2251799813685248) in
+           expr_let y46 := Z.modulo @@ (y44, 2251799813685248) in
+           expr_let _ := Z.div @@ (y36, 2251799813685248) in
+           expr_let _ := Z.modulo @@ (y36, 2251799813685248) in
+           expr_let _ := Z.div @@ (y25, 2251799813685248) in
+           expr_let _ := Z.modulo @@ (y25, 2251799813685248) in
+           expr_let _ := Z.div @@ (y13, 2251799813685248) in
+           expr_let _ := Z.modulo @@ (y13, 2251799813685248) in
            expr_let y53 := y45 +
-                           (x [[0]] * x0 [[4]] +
-                            (x [[1]] * x0 [[3]] +
-                             (x [[2]] * x0 [[2]] +
-                              (x [[3]] * x0 [[1]] + x [[4]] * x0 [[0]])))) in
-           expr_let _ := Ident ident.Z.div @ y53 @ 2251799813685248 in
-           expr_let _ := Ident ident.Z.modulo @ y53 @ 2251799813685248 in
-           expr_let _ := Ident ident.Z.div @ y46 @ 2251799813685248 in
-           expr_let _ := Ident ident.Z.modulo @ y46 @ 2251799813685248 in
-           expr_let _ := Ident ident.Z.div @ y36 @ 2251799813685248 in
-           expr_let _ := Ident ident.Z.modulo @ y36 @ 2251799813685248 in
-           expr_let _ := Ident ident.Z.div @ y25 @ 2251799813685248 in
-           expr_let _ := Ident ident.Z.modulo @ y25 @ 2251799813685248 in
-           expr_let y62 := Ident ident.Z.div @ y13 @ 2251799813685248 in
-           expr_let y63 := Ident ident.Z.modulo @ y13 @ 2251799813685248 in
+                           (fst @@ x [[0]] * snd @@ x [[4]] +
+                            (fst @@ x [[1]] * snd @@ x [[3]] +
+                             (fst @@ x [[2]] * snd @@ x [[2]] +
+                              (fst @@ x [[3]] * snd @@ x [[1]] +
+                               fst @@ x [[4]] * snd @@ x [[0]])))) in
+           expr_let _ := Z.div @@ (y53, 2251799813685248) in
+           expr_let _ := Z.modulo @@ (y53, 2251799813685248) in
+           expr_let _ := Z.div @@ (y46, 2251799813685248) in
+           expr_let _ := Z.modulo @@ (y46, 2251799813685248) in
+           expr_let _ := Z.div @@ (y36, 2251799813685248) in
+           expr_let _ := Z.modulo @@ (y36, 2251799813685248) in
+           expr_let _ := Z.div @@ (y25, 2251799813685248) in
+           expr_let _ := Z.modulo @@ (y25, 2251799813685248) in
+           expr_let y62 := Z.div @@ (y13, 2251799813685248) in
+           expr_let y63 := Z.modulo @@ (y13, 2251799813685248) in
            expr_let y64 := y45 +
-                           (x [[0]] * x0 [[4]] +
-                            (x [[1]] * x0 [[3]] +
-                             (x [[2]] * x0 [[2]] +
-                              (x [[3]] * x0 [[1]] + x [[4]] * x0 [[0]])))) in
-           expr_let _ := Ident ident.Z.div @ y64 @ 2251799813685248 in
-           expr_let _ := Ident ident.Z.modulo @ y64 @ 2251799813685248 in
-           expr_let _ := Ident ident.Z.div @ y46 @ 2251799813685248 in
-           expr_let _ := Ident ident.Z.modulo @ y46 @ 2251799813685248 in
-           expr_let _ := Ident ident.Z.div @ y36 @ 2251799813685248 in
-           expr_let _ := Ident ident.Z.modulo @ y36 @ 2251799813685248 in
+                           (fst @@ x [[0]] * snd @@ x [[4]] +
+                            (fst @@ x [[1]] * snd @@ x [[3]] +
+                             (fst @@ x [[2]] * snd @@ x [[2]] +
+                              (fst @@ x [[3]] * snd @@ x [[1]] +
+                               fst @@ x [[4]] * snd @@ x [[0]])))) in
+           expr_let _ := Z.div @@ (y64, 2251799813685248) in
+           expr_let _ := Z.modulo @@ (y64, 2251799813685248) in
+           expr_let _ := Z.div @@ (y46, 2251799813685248) in
+           expr_let _ := Z.modulo @@ (y46, 2251799813685248) in
+           expr_let _ := Z.div @@ (y36, 2251799813685248) in
+           expr_let _ := Z.modulo @@ (y36, 2251799813685248) in
            expr_let y71 := y62 + y25 in
-           expr_let y72 := Ident ident.Z.div @ y71 @ 2251799813685248 in
-           expr_let y73 := Ident ident.Z.modulo @ y71 @ 2251799813685248 in
-           expr_let _ := Ident ident.Z.div @ y63 @ 2251799813685248 in
-           expr_let _ := Ident ident.Z.modulo @ y63 @ 2251799813685248 in
+           expr_let y72 := Z.div @@ (y71, 2251799813685248) in
+           expr_let y73 := Z.modulo @@ (y71, 2251799813685248) in
+           expr_let _ := Z.div @@ (y63, 2251799813685248) in
+           expr_let _ := Z.modulo @@ (y63, 2251799813685248) in
            y63
            :: y73
               :: y72 + y36
                  :: y46
                     :: y45 +
-                       (x [[0]] * x0 [[4]] +
-                        (x [[1]] * x0 [[3]] +
-                         (x [[2]] * x0 [[2]] +
-                          (x [[3]] * x0 [[1]] + x [[4]] * x0 [[0]])))) :: [])%expr)
-         f g
-     : forall f g : list Z, length f = 5%nat -> length g = 5%nat -> list Z
-*)
+                       (fst @@ x [[0]] * snd @@ x [[4]] +
+                        (fst @@ x [[1]] * snd @@ x [[3]] +
+                         (fst @@ x [[2]] * snd @@ x [[2]] +
+                          (fst @@ x [[3]] * snd @@ x [[1]] +
+                           fst @@ x [[4]] * snd @@ x [[0]])))) :: [])%expr) fg
+     : forall fg : list Z * list Z,
+       length (Datatypes.fst fg) = 5%nat ->
+       length (Datatypes.snd fg) = 5%nat -> list Z *)
